
@prefix lti: <http://ld.kinexis.com/vocab/lti/v2/lti#> .
@prefix xsd: <http://www.w3.org/2001/XMLSchema#> .
@prefix owl: <http://www.w3.org/2002/07/owl#> .
@prefix lti-type: <http://ld.kinexis.com/xsd/lti/v2/ltid#> .
@prefix liso: <http://ld.kinexis.com/vocab/lis/v2/outcomes#> .
@prefix org: <http://www.w3.org/ns/org#> .
@prefix rdf: <http://www.w3.org/1999/02/22-rdf-syntax-ns#> .
@prefix rdfs: <http://www.w3.org/2000/01/rdf-schema#> .
@prefix bind: <http://purl.org/semantictools/v1/vocab/bind#> .

<http://ld.kinexis.com/vocab/lti/v2/lti#> a owl:Ontology  ;
  rdfs:label "LTI Core" ;
  a bind:TargetNamespace ;
  bind:suggestedPrefix "lti" .

lti:BaseUrlChoice rdf:type owl:Class;
  rdfs:subClassOf 
  [ a owl:Restriction ;
    owl:onProperty      lti:default_base_url;
    owl:minCardinality  1;
    rdfs:comment "This is the base URL that should be used by default for all entities specified by the associated BaseUrlSelector.  The secure_base_url attribute may override this default Base URL."
  ] ,
  [ a owl:Restriction ;
    owl:onProperty      lti:secure_base_url;
    rdfs:comment "This is the base URL that should be used whenever security is enabled.  If this base URL is not defined, then the default_base_url is used in all circumstances."
  ] ,
  [ a owl:Restriction ;
    owl:onProperty      lti:selector;
    rdfs:comment "A resource that specifies the objects to which this BaseUrlChoice applies. "
  ] ; 
  rdfs:comment "Defines the base URL that is used for certain kinds of resources referenced in a ToolProfile.  The kinds of resources to which the base URL applies is specified by an associated BaseUrlSelector.  If the BaseUrlChoice does not have an associated selector, then it applies universally to all resources referenced in the Tool Profile. " .

lti:BaseUrlSelector rdf:type owl:Class;
  rdfs:subClassOf 
  [ a owl:Restriction ;
    owl:onProperty      lti:applies_to;
    owl:minCardinality  1;
    rdfs:comment "The class of resources selected by this BaseUrlSelector."
  ] ; 
  rdfs:comment "This resource specifies the type of objects to which a set of base URLs apply. " .

lti:Contact rdf:type owl:Class;
  rdfs:subClassOf 
  [ a owl:Restriction ;
    owl:onProperty      lti:email;
    owl:minCardinality  1;
    rdfs:comment "The email of the primary contact for the associated object."
  ] ; 
  rdfs:comment "Contact information for the associated object." .

lti:Endpoint rdf:type owl:Class;
  rdfs:subClassOf 
  [ a owl:Restriction ;
    owl:onProperty      lti:path;
    owl:minCardinality  1;
    rdfs:comment """This attribute specifies the path for an endpoint such as a MessageHandler or an Icon. Typically, this path is relative to one of the base URL values defined in a BaseUrlChoice.  
In the case of a MessageHandler, the path may be an absolute path if the associated message type explicitly declares that an absolute path is allowed.  """
  ] ; 
  rdfs:comment "This is the abstract base class for objects that have an endpoint such as icons or message handlers. " .

lti:ServiceProvider rdf:type owl:Class;
  rdfs:subClassOf 
  [ a owl:Restriction ;
    owl:onProperty      lti:guid;
    owl:minCardinality  1;
    rdfs:comment "A globally unique identifier for the service provider.  As a best practice, this value should match an Internet domain name assigned by ICANN, but any globally unique identifier is acceptable.  "
  ] ,
  [ a owl:Restriction ;
    owl:onProperty      lti:timestamp;
    owl:minCardinality  1;
    rdfs:comment "A timestamp for the ServiceProvider record. This value is useful for determining which record is most current."
  ] ,
  [ a owl:Restriction ;
    owl:onProperty      lti:service_provider_name;
    owl:minCardinality  1;
    rdfs:comment "The name of the service provider, suitable for display to end users."
  ] ,
  [ a owl:Restriction ;
    owl:onProperty      lti:description;
    rdfs:comment "A description of the service provider, suitable for display to end-users."
  ] ,
  [ a owl:Restriction ;
    owl:onProperty      lti:support;
    rdfs:comment "Contact information for support from a service provider."
  ] ; 
  rdfs:comment "This resource represents the service provider that hosts a product (Tool or Tool Consumer)." .

lti:IconEndpoint rdf:type owl:Class ;
  rdfs:subClassOf lti:Endpoint ; 
  rdfs:comment "Defines the path for an Icon.  " .

lti:IconInfo rdf:type owl:Class;
  rdfs:subClassOf 
  [ a owl:Restriction ;
    owl:onProperty      lti:key;
    rdfs:comment "If localization is supported then the 'key' attribute identifies a property in the resource bundle provided in response to the get-bundle-request message. The value of that property is the locale-specific path to the icon."
  ] ,
  [ a owl:Restriction ;
    owl:onProperty      lti:default_location;
    rdfs:comment "Specifies the default path to an icon.  The absolute URL is formed by appending this path to the appropriate base URL for icons."
  ] ,
  [ a owl:Restriction ;
    owl:onProperty      lti:icon_style;
    rdfs:comment "The style of the icon referenced by this IconInfo."
  ] ; 
  rdfs:comment "Contains information about a graphical icon that may be displayed in the Tool Consumer's user interface." .

lti:IconStyle rdf:type owl:Class ; 
  rdfs:comment """<p>A resource that specifies the style for an Icon.</p>
The LTI standard does not define any particular Icon styles.  Each vendor is free to publish its own set of icon styles.  A typical style might specify dimensions of the icon or its intended usage.  Each IconStyle is uniquely identified by a URI.  Ideally, the URI should resolve to a resource that provides a definition of the icon style.""" .

lti:LocalizedName rdf:type owl:Class;
  rdfs:subClassOf 
  [ a owl:Restriction ;
    owl:onProperty      lti:key;
    rdfs:comment "The key used to lookup the locale-specific value from a resource bundle."
  ] ,
  [ a owl:Restriction ;
    owl:onProperty      lti:default_value;
    owl:allValuesFrom  lti-type:LongName.Type;
    rdfs:comment "The default value for the display name.  This value is used if (1) the key attribute is undefined, (2) the localization capability is not enabled, or (3) a value for the specified key is not found in the locale-specific resource bundle."
  ] ; 
  rdfs:comment "This container stores the default display name for some object plus a key that may be used to lookup a translation for the display name from a resource bundle for a particular locale.  The string value has a maximum length of 128 characters." .

lti:LocalizedText rdf:type owl:Class;
  rdfs:subClassOf 
  [ a owl:Restriction ;
    owl:onProperty      lti:key;
    rdfs:comment "If localization is supported then the key identifies a property in the bundle returned by the get-bundle-request message handler. "
  ] ,
  [ a owl:Restriction ;
    owl:onProperty      lti:default_value;
    owl:allValuesFrom  lti-type:Text.Type;
    rdfs:comment "This is the default value for the text. This default value  is used if (1) the key is not specified, (2) the localization capability is not enabled, or (3) the specified key is not found in the locale-specific resource bundle."
  ] ; 
  rdfs:comment "This container defines a block of text.  The container includes a default value for the text, plus a key that can be used to lookup a locale-specific value from a resource bundle." .

lti:MessageHandler rdf:type owl:Class ;
  rdfs:subClassOf lti:Endpoint ,
  [ a owl:Restriction ;
    owl:onProperty      lti:enabled_capability;
    rdfs:comment "A capability that is enabled for messages handled by this MessageHandler."
  ] ,
  [ a owl:Restriction ;
    owl:onProperty      lti:message_type;
    owl:minCardinality  1;
    rdfs:comment "The type of message that can be submitted to the Message Handler."
  ] ,
  [ a owl:Restriction ;
    owl:onProperty      lti:parameter;
    rdfs:comment "Specifies a custom parameter that is expected by the MessageHandler."
  ] ; 
  rdfs:comment "Defines the features of a message handler, including information about the handler's service endpoint and custom parameters that it expects." .

lti:ProductInfo rdf:type owl:Class;
  rdfs:subClassOf 
  [ a owl:Restriction ;
    owl:onProperty      lti:product_name;
    owl:minCardinality  1;
    rdfs:comment "A name for the product, suitable for display to end users."
  ] ,
  [ a owl:Restriction ;
    owl:onProperty      lti:product_version;
    owl:minCardinality  1;
    rdfs:comment "This is the version of the product. "
  ] ,
  [ a owl:Restriction ;
    owl:onProperty      lti:description;
    rdfs:comment "This is a description of the product suitable for display to end-users."
  ] ,
  [ a owl:Restriction ;
    owl:onProperty      lti:technical_description;
    rdfs:comment "This is a human readable description of the technical aspects of this product that might be of interest to developers who wish to integrate with this product via LTI."
  ] ,
  [ a owl:Restriction ;
    owl:onProperty      lti:product_family;
    owl:minCardinality  1;
    rdfs:comment "An inverse attribute that references the ProductFamily within which this ProductInfo is defined."
  ] ,
  [ a owl:Restriction ;
    owl:onProperty      lti:instance;
    rdfs:comment "A deployed instance of a particular version of a product (Tool or Tool Consumer)."
  ] ; 
  rdfs:comment "Encapsulates information about one released version of a product (Tool Consumer or Tool)." .

lti:ProductFamily rdf:type owl:Class ;
  rdfs:subClassOf lti:HasCode ,
  [ a owl:Restriction ;
    owl:onProperty      lti:vendor;
    owl:minCardinality  1;
    rdfs:comment "The vendor that owns the ProductFamily."
  ] ,
  [ a owl:Restriction ;
    owl:onProperty      lti:version;
    rdfs:comment "Encapsulates information about one version of the product."
  ] ; 
  rdfs:comment """A ProductFamily represents the collection of all versions of a particular product over time.  Two products that have the same product <em>code</em> belong to the same ProductFamily.  The LTI product model has four levels: <OL>
  <LI> <code>ProductFamily</code>:  The collection of all versions of a given product.
  <LI> <code>ProductInfo</code>: Encapsulates information about one particular version of a product.
  <LI> <code>ProductInstance</code>: Represents one deployed instance of a particular version of a product.
  <LI> <code>ProductProfile</code>: Defines a <em>view</em> of a deployed instance of a product.  This view may be customized for different integration partners.
</OL>

Notice that the ProductFamily sits at the top of the product hierarchy.  Each product family is owned by a <code>Vendor</code>.""" .

lti:ProductProfile rdf:type owl:Class;
  rdfs:subClassOf 
  [ a owl:Restriction ;
    owl:onProperty      lti:lti_version;
    owl:allValuesFrom  xsd:normalizedString;
    owl:minCardinality  1;
    rdfs:comment "The identifier for an LTI version that the version supports.  A given product (Tool or Tool Consumer) may support multiple versions, but only one version is selected for use in the integration contract."
  ] ,
  [ a owl:Restriction ;
    owl:onProperty      lti:service_offered;
    rdfs:comment "The descriptor for a service offered by the product (Tool or Tool Consumer)."
  ] ,
  [ a owl:Restriction ;
    owl:onProperty      lti:product_instance;
    owl:minCardinality  1;
    rdfs:comment "An inverse attribute which references the ProductInstance within which this ProductProfile is defined."
  ] ; 
  rdfs:comment """A ProductProfile presents an integration view of a deployed instance of some product (Tool or Tool Consumer).  It defines the services and other features offered to an integration partner.  A profile may be customized for each integration partner or shared with multiple partners.
<p>ProductProfile is the abstract base class for all product profiles. The ToolConsumerProfile and ToolProfile are derived from this base class.  </p>""" .

lti:ServiceDescriptor rdf:type owl:Class ; 
  rdfs:comment """This entity defines a profile for a service.  It is a \"profile\" in the sense that it specifies a subset of operations that are declared by the full  interface for some service.  For example, a profile might list the \"read\" operations of a service but exclude the \"write\" operations.  This is useful because a product (Tool or TC) might want to offer the read-only operations to a partner, but it might not want to expose write operations.  (On the other hand, it is perfectly legitimate for a profile to list all of the operations that are declared in the service interface if desired.)
ServiceProfiles are used for four different purposes: (1) they allow a product to advertise the operations that it offers to a partner, (2) they allow a product to declare the operations that it intends to use, (3) they allow a product to advertise the security profiles that are available for service operations, and (4) they allow a product to assert the security profiles that will be used for service operations. """ .

lti:ToolConsumerProfile rdf:type owl:Class ;
  rdfs:subClassOf lti:ProductProfile ,
  [ a owl:Restriction ;
    owl:onProperty      lti:guid;
    owl:minCardinality  1
  ] ,
  [ a owl:Restriction ;
    owl:onProperty      lti:capability_offered;
    rdfs:comment "A capability offered by the Tool Consumer to its integration partners."
  ] ; 
  rdfs:comment "The profile for a Tool Consumer product." .

lti:ToolProfile rdf:type owl:Class ;
  rdfs:subClassOf lti:ProductProfile ,
  [ a owl:Restriction ;
    owl:onProperty      lti:message;
    rdfs:comment "A definition of a message supported by the resource handler."
  ] ,
  [ a owl:Restriction ;
    owl:onProperty      lti:resource_handler;
    rdfs:comment "A definition of a resource offered by the tool provider."
  ] ,
  [ a owl:Restriction ;
    owl:onProperty      lti:base_url_choice;
    owl:minCardinality  1;
    rdfs:comment "Base URLs to use as a prefix to any incomplete URLs specified in the diocument."
  ] ; 
  rdfs:comment "The profile for a Tool product." .

lti:ResourceHandler rdf:type owl:Class;
  rdfs:subClassOf 
  [ a owl:Restriction ;
    owl:onProperty      lti:resource_name;
    owl:minCardinality  1;
    rdfs:comment "The name of the resource handler suitable for display in the TC user interface."
  ] ,
  [ a owl:Restriction ;
    owl:onProperty      lti:resource_type;
    owl:minCardinality  1;
    rdfs:comment "Identifies the type of resource associated with this ResourceHandler.  Resource types are identified by a code that is unique within a given ProductFamily."
  ] ,
  [ a owl:Restriction ;
    owl:onProperty      lti:message;
    owl:minCardinality  1;
    rdfs:comment "Defines the features of a message handler associated with the resource described by this ResourceHandler."
  ] ,
  [ a owl:Restriction ;
    owl:onProperty      lti:icon_info;
    rdfs:comment "Provides information about a graphical icon that represents the resource described by this ResourceHandler."
  ] ; 
  rdfs:comment "The set of information for a specific resource handler." .

lti:Parameter rdf:type owl:Class;
  rdfs:subClassOf 
  [ a owl:Restriction ;
    owl:onProperty      lti:name;
    owl:minCardinality  1;
    rdfs:comment "The name of the parameter."
  ] ,
  [ a owl:Restriction ;
    owl:onProperty      lti:fixed;
    rdfs:comment "Denotes that the value of the parameter is fixed at the time of definition within the product profile.  This value must be passed in each message of the associated message type."
  ] ,
  [ a owl:Restriction ;
    owl:onProperty      lti:variable;
    rdfs:comment "Denotes that the parameter has a variable value that is automatically substituted at run-time.  The value of this attribute is the name for a variable whose value will be added to the message at run-time. "
  ] ; 
  rdfs:comment "Defines the characteristics of a parameter expected by a MessageHandler." .

lti:ShortLocalizedName rdf:type owl:Class;
  rdfs:subClassOf 
  [ a owl:Restriction ;
    owl:onProperty      lti:key;
    rdfs:comment "The key used to lookup the locale-specific value from a resource bundle."
  ] ,
  [ a owl:Restriction ;
    owl:onProperty      lti:default_value;
    owl:allValuesFrom  lti-type:ShortName.Type;
    rdfs:comment "The default value for the display name.  This value is used if (1) the key attribute is undefined, (2) the localization capability is not enabled, or (3) a value for the specified key is not found in the locale-specific resource bundle."
  ] ; 
  rdfs:comment "This container stores the default display name for some object plus a key that may be used to lookup a translation for the display name from a resource bundle for a particular locale.  This class is similar to LocalizedName, except that that the string value is limited to 64 characters." .

lti:Vendor rdf:type owl:Class ;
  rdfs:subClassOf lti:HasCode ,
  [ a owl:Restriction ;
    owl:onProperty      lti:timestamp;
    owl:minCardinality  1;
    rdfs:comment "A timestamp for the Vendor record. This value is useful for determining which record is most current."
  ] ,
  [ a owl:Restriction ;
    owl:onProperty      lti:vendor_name;
    owl:minCardinality  1;
    rdfs:comment "Defines a human readable name for the Vendor.  The name should be suitable for display in management screens within the Tool Provider system."
  ] ,
  [ a owl:Restriction ;
    owl:onProperty      lti:description;
    rdfs:comment "This is a human-readable description of the Vendor."
  ] ,
  [ a owl:Restriction ;
    owl:onProperty      lti:website;
    rdfs:comment "This is the URL of the vendor."
  ] ,
  [ a owl:Restriction ;
    owl:onProperty      lti:product;
    rdfs:comment """<p>A group of related products offered by the Vendor.  All of the products within a given product family are different <em>versions</em> of the same product. </p>
<p>A vendor may have multiple product families.  For example, the same vendor might offer a discussion forum tool and also a white board tool.  Each of these tools corresponds to a different product family.</p>"""
  ] ,
  [ a owl:Restriction ;
    owl:onProperty      lti:contact;
    rdfs:comment "Contact information for this Vendor."
  ] ; 
  rdfs:comment "A person or agency that offers products to the market. The key types of products relevant to LTI are Tools (which are described by Tool Profiles) and Tool Consumers (which are described by Tool Consumer Profiles)." .

lti:Capability rdf:type owl:Class ; 
  rdfs:comment "Represents a capability that may be declared by a Tool Consumer in its profile and enabled by a Tool when an integration contract is established." .

lti:MessageType rdf:type owl:Class ;
  rdfs:subClassOf lti:Capability ,
  [ a owl:Restriction ;
    owl:onProperty      lti:absolute_path_allowed;
    rdfs:comment "Specifies whether the path for this message type is allowed to be specified using an absolute path.  A value of \"false\" means that the MessageHandler must declare a relative path."
  ] ,
  [ a owl:Restriction ;
    owl:onProperty      lti:message_class;
    owl:minCardinality  1;
    rdfs:comment "This attribute identifies the formal Class definition the type of message that can be delivered to a given MessageHandler."
  ] ,
  [ a owl:Restriction ;
    owl:onProperty      lti:http_method;
    owl:minCardinality  1;
    rdfs:comment "Specifies an HTTP method (POST, GET, PUT, etc.) for the type of messages represented by this MessageType."
  ] ; 
  rdfs:comment """This container holds metadata about a particular type of message.
It provides a friendly name (an alias) for the formal Message class name, and it specifies the allowed HTTP methods for Messages of the given type.""" .

lti:SecurityContract rdf:type owl:Class;
  rdfs:subClassOf 
  [ a owl:Restriction ;
    owl:onProperty      lti:shared_secret;
    owl:minCardinality  1;
    rdfs:comment """This is the shared secret used for communications between the Tool Consumer and the Tool Provider.  It is expected that the Tool Consumer present an interface to the administrative user for them to activate the Tool Proxy before this secret is ever used by the Tool Consumer. 
The shared secret may be updated when a tool is re-registered (see the reregisterTool operation of the ToolRegistrationService).  In addition, the TC and TP should provide interfaces which allow their respective administrators to change the shared secret through an out-of-band agreement."""
  ] ,
  [ a owl:Restriction ;
    owl:onProperty      lti:tool_service;
    rdfs:comment "The profile for a Tool Consumer service that may be invoked by the Tool acting on its own (as opposed to acting as an agent for some end user).  "
  ] ,
  [ a owl:Restriction ;
    owl:onProperty      lti:end_user_service;
    rdfs:comment "The profile for a Tool Consumer service that may be invoked by the Tool when acting as an agent for some end user.  "
  ] ; 
  rdfs:comment """This entity specifies all aspects of the security agreements between Tool Provider and Tool Consumer.
<p>
Notice that the security contract distinguishes between <code>tool_service</code>s and <code>end_user_service</code>s.  A <code>tool_service</code> is a service that the Tool invokes when acting on its own.  By contrast, a <code>end_user_service</code> is a service that the Tool invokes when acting as an agent for some end user.  Consider, for example, the case where a Tool is reporting scores to the Tool Consumer via an outcomes service.  When a student submits an assignment, the Tool may calculate a score and post it to the Tool Consumer.  In this case the Tool is acting on its own since students generally do not have permission to enter their own scores into a grade book.  Now, suppose the Tool exposes a user interface which allows instructors to change a score.  In this case, when the Tool posts the modified score to the Tool Consumer grade book, it is acting as an agent for the end user.  This example, illustrates that the same service may be referenced as both a <code>tool_service</code> and a <code>end_user_service</code>
</p>
""" .

lti:ServiceProfile rdf:type owl:Class;
  rdfs:subClassOf 
  [ a owl:Restriction ;
    owl:onProperty      lti:service;
    owl:minCardinality  1;
    rdfs:comment "The descriptor for the service that is being profiled."
  ] ; 
  rdfs:comment "A profile for some service that may be invoked by an integration partner.  A profile specifies which methods or operations the integration partner intends to use." .

lti:RestServiceProfile rdf:type owl:Class ;
  rdfs:subClassOf lti:ServiceProfile ,
  [ a owl:Restriction ;
    owl:onProperty      lti:action;
    owl:minCardinality  1;
    rdfs:comment "Specifies an HTTP method (POST, GET, PUT, etc.) which the integration partner intends to use.   A RestServiceProfile may include more than one action.  However, the set of actions declared in a RestServiceProfile must be a subset of actions declared in the RestService referenced by the <code>service</code> property."
  ] ; 
  rdfs:comment "A kind of ServiceProfile specialized for REST services. " .

lti:ResourceType rdf:type owl:Class ;
  rdfs:subClassOf lti:HasCode ,
  [ a owl:Restriction ;
    owl:onProperty      lti:resource_type_owner;
    owl:minCardinality  1
  ] ; 
  rdfs:comment "This class represents all ResourceHandlers of a given type.  Two ResourceHandlers that belong to this set are considered to be different versions of the same ResourceHandler." .

lti:HasCode rdf:type owl:Class;
  rdfs:subClassOf 
  [ a owl:Restriction ;
    owl:onProperty      lti:code;
    owl:minCardinality  1;
    rdfs:comment "A unique identifier for the resource."
  ] ; 
  rdfs:comment "A resource that can be identified by a <code>code</code> property.  The code property may be globally unique (as in the case of a Vendor resource) or locally unqiue (as in the case of a Product Family, where the code is locally unique within the scope of the parent Vendor resource)." .

lti:RestService rdf:type owl:Class ;
  rdfs:subClassOf lti:ServiceDescriptor ,
  [ a owl:Restriction ;
    owl:onProperty      lti:format;
    owl:minCardinality  1;
    rdfs:comment "The content type (also known as media type) of resources accessed via the endpoint defined by this RestService descriptor.   The endpoint of a REST service may support more than one content type if content negotiation is enabled as described in the <a href=\"http://www.w3.org/Protocols/rfc2616/rfc2616-sec12.html\">HTTP 1.1</a> specification."
  ] ,
  [ a owl:Restriction ;
    owl:onProperty      lti:endpoint;
    owl:minCardinality  1;
    rdfs:comment "A URI template that defines the REST endpoint for resources that may be accessed via the REST service.  The URI template should conform to the syntax in the proposed IETF standard [<a href=\"http://www.ietf.org/id/draft-gregorio-uritemplate-08.txt\">draft-gregorio-uritemplate-08</a>]. "
  ] ,
  [ a owl:Restriction ;
    owl:onProperty      lti:action;
    owl:minCardinality  1;
    rdfs:comment "Specifies an HTTP action that is supported at the REST endpoint.  A given endpoint may support more than one action.  For example, it is common practice for a collection endpoint to accept POST requests, and a different item endpoint to accept GET, PUT, and DELETE requests."
  ] ; 
  rdfs:comment "A descriptor for a REST service." .

lti:ProductInstance rdf:type owl:Class;
  rdfs:subClassOf 
  [ a owl:Restriction ;
    owl:onProperty      lti:guid;
    owl:minCardinality  1
  ] ,
  [ a owl:Restriction ;
    owl:onProperty      lti:service_provider;
    rdfs:comment "This is the service provider that hosts the deployed product."
  ] ,
  [ a owl:Restriction ;
    owl:onProperty      lti:product_info;
    owl:minCardinality  1;
    rdfs:comment "This is metadata about the product described in the profile."
  ] ,
  [ a owl:Restriction ;
    owl:onProperty      lti:profile;
    rdfs:comment "A resource that presents a view of this ProductInstance to one or more integration partners."
  ] ,
  [ a owl:Restriction ;
    owl:onProperty      lti:support;
    rdfs:comment "Contact information for support on this deployed instance of the product (Tool or ToolConsumer)."
  ] ,
  [ a owl:Restriction ;
    owl:onProperty      lti:service_owner;
    rdfs:comment "The entity that owns the services provided by this product instance."
  ] ; 
  rdfs:comment "The resource encapsulates information about one deployed instance of a web-based product (Tool or Tool Consumer)." .

lti:ServiceOwner rdf:type owl:Class;
  rdfs:subClassOf 
  [ a owl:Restriction ;
    owl:onProperty      lti:timestamp;
    owl:minCardinality  1;
    rdfs:comment "A timestamp for the ServiceOwner record. This value is useful for determining which record is most current."
  ] ,
  [ a owl:Restriction ;
    owl:onProperty      lti:service_owner_name;
    owl:minCardinality  1;
    rdfs:comment "The name of the service owner, suitable for display to end users. "
  ] ,
  [ a owl:Restriction ;
    owl:onProperty      lti:description;
    rdfs:comment "A description of the service owner, suitable for display to end-users."
  ] ; 
  rdfs:comment "The entity that owns the services provided by a product instance." .

lti:ToolProxy rdf:type owl:Class ;
  rdfs:subClassOf lti:ToolSettingsContainer ,
  [ a owl:Restriction ;
    owl:onProperty      lti:lti_version;
    owl:allValuesFrom  xsd:token;
    owl:minCardinality  1;
    rdfs:comment "The LTI version that governs the integration between the Tool and ToolConsumer. "
  ] ,
  [ a owl:Restriction ;
    owl:onProperty      lti:tool_proxy_guid;
    owl:minCardinality  1;
    rdfs:comment "The globally unique identifier for the ToolProxy (a.k.a. integration contract)."
  ] ,
  [ a owl:Restriction ;
    owl:onProperty      lti:tool_profile;
    owl:minCardinality  1;
    rdfs:comment "The profile of the Tool that is participating in the integration governed by this ToolProxy."
  ] ,
  [ a owl:Restriction ;
    owl:onProperty      lti:security_contract;
    owl:minCardinality  1;
    rdfs:comment "The security aspect of an integration contract between two parties."
  ] ,
  [ a owl:Restriction ;
    owl:onProperty      lti:tool_consumer_profile;
    owl:minCardinality  1;
    rdfs:comment "The profile of the Tool Consumer that is participating in the integration governed by this ToolProxy."
  ] ; 
  rdfs:comment "This entity defines the integration contract between a ToolConsumer and a Tool.   It is called a \"ToolProxy\" because its primary purpose is to provide the ToolConsumer with all of the information needed to embed a given Tool within the ToolConsumer system." .

lti:ToolProxyBinding rdf:type owl:Class ;
  rdfs:subClassOf lti:ToolSettingsContainer ,
  [ a owl:Restriction ;
    owl:onProperty      lti:context;
    owl:minCardinality  1;
    rdfs:comment "The learning Context associated with this <code>ToolProxyBinding</code>."
  ] ; 
  rdfs:comment "A <code>ToolProxyBinding</code> associates a ToolProxy with a learning Context (such as a Course Section).   This association must be established before the corresponding Tool can be used within the Context.  The <code>ToolProxyBinding</code> also serves as a container that holds tool settings associated with the learning Context." .

lti:ResourceLink rdf:type owl:Class;
  rdfs:subClassOf 
  [ a owl:Restriction ;
    owl:onProperty      lti:resourceLinkId;
    owl:minCardinality  1;
    rdfs:comment "A globally unique identifier for this LTI link."
  ] ; 
  rdfs:comment "An <code>LtiLink</code> represents a link within the Tool Consumer system pointing to a resource within the Tool Provider." .

lti:Context rdf:type owl:Class ;
  rdfs:subClassOf org:Organization ,
  [ a owl:Restriction ;
    owl:onProperty      lti:contextId;
    owl:minCardinality  1;
    rdfs:comment "A unique string provided by the tool consumer to identify the context (as passed in the context_id launch parameter)."
  ] ,
  [ a owl:Restriction ;
    owl:onProperty      lti:sourcedId;
    rdfs:comment "A unique identifier for the context as provisioned by an external system such as an SIS."
  ] ,
  [ a owl:Restriction ;
    owl:onProperty      lti:lineItem;
    rdfs:comment "A LineItem that records results for some learning activity within this context."
  ] ,
  [ a owl:Restriction ;
    owl:onProperty      lti:lineItems;
    rdfs:comment """The container that holds the collection of LineItem resources for this Context.  In general, this container is optional.  However, if the Context has any associated LineItems, then the container is required.  As a best practice, implementations every Context should expose a LineItemContainer to clients, even if it is empty.
"""
  ] ; 
  rdfs:comment "A learning context, such as a Course Section." .

lti:ToolSettingsContainer rdf:type owl:Class;
  rdfs:subClassOf 
  [ a owl:Restriction ;
    owl:onProperty      lti:custom;
    rdfs:comment "A collection of custom properties defined by the Tool Provider and stored in this ToolSettingsContainer."
  ] ; 
  rdfs:comment "<code>ToolSettingsContainer</code> is the base class for all resources that encapsulate tool settings." .

lti:PropertyMap rdf:type owl:Class ; 
  rdfs:comment "An abstract class whose properties are defined by the Tool Provider and stored in the Tool Consumer.   When represented in JSON-LD, the PropertyMap object typically appears as a plain-old JSON object (though it may have a custom JSON-LD context that defines the semantics for the custom properties).  It is a best practice for the values in a PropertyMap to be strings.  This best practice may be revised if the development community expresses a desire to support other data types in a PropertyMap." .

lti:LtiLink rdf:type owl:Class ;
  rdfs:subClassOf lti:ToolSettingsContainer ,
  [ a owl:Restriction ;
    owl:onProperty      lti:settingsResourceLink;
    owl:minCardinality  1;
    rdfs:comment "The resource link associated with the settings."
  ] .

lti:DocumentTarget rdf:type owl:Class .

lti:HttpMethod a owl:Class  ;
  owl:equivalentClass [
    owl:oneOf (
      lti:GET 
      lti:POST 
      lti:PUT 
      lti:DELETE
    )
  ] ;
  rdfs:comment "Enumerates the HTTP methods that can be used when sending a message, as defined by IETF RFC 2616 ." .

lti:default_base_url rdf:type owl:FunctionalProperty ;
  rdfs:domain lti:BaseUrlChoice ;
  rdfs:range xsd:anyURI ;
  rdfs:comment "This is the base URL that should be used by default for all entities specified by the associated BaseUrlSelector.  The secure_base_url attribute may override this default Base URL." .

lti:secure_base_url rdf:type owl:FunctionalProperty ;
  rdfs:domain lti:BaseUrlChoice ;
  rdfs:range xsd:anyURI ;
  rdfs:comment "This is the base URL that should be used whenever security is enabled.  If this base URL is not defined, then the default_base_url is used in all circumstances." .

lti:selector rdf:type owl:FunctionalProperty ;
  rdfs:domain lti:BaseUrlChoice ;
  rdfs:range lti:BaseUrlSelector ;
  rdfs:comment "A resource that specifies the objects to which this BaseUrlChoice applies. " .

lti:applies_to rdf:type rdf:Property ;
  rdfs:domain lti:BaseUrlSelector ;
  rdfs:range owl:Class ;
  rdfs:comment "The class of resources selected by this BaseUrlSelector." .

lti:email rdf:type owl:FunctionalProperty ;
  rdfs:domain lti:Contact ;
  rdfs:range xsd:normalizedString ;
  rdfs:comment "The email of the primary contact for the associated object." .

lti:path rdf:type owl:FunctionalProperty ;
  rdfs:domain lti:Endpoint ;
  rdfs:range xsd:anyURI ;
  rdfs:comment """This attribute specifies the path for an endpoint such as a MessageHandler or an Icon. Typically, this path is relative to one of the base URL values defined in a BaseUrlChoice.  
In the case of a MessageHandler, the path may be an absolute path if the associated message type explicitly declares that an absolute path is allowed.  """ .

lti:guid rdf:type owl:FunctionalProperty ;
  rdfs:domain  [
    rdf:type owl:Class ;
    owl:unionOf (
      lti:ServiceProvider
      lti:ToolConsumerProfile
      lti:ProductInstance
    )
  ] ;
  rdfs:range lti-type:GUID.Type ;
  rdfs:comment "A globally unique identifier for the service provider.  As a best practice, this value should match an Internet domain name assigned by ICANN, but any globally unique identifier is acceptable.  " .

lti:timestamp rdf:type owl:FunctionalProperty ;
  rdfs:domain  [
    rdf:type owl:Class ;
    owl:unionOf (
      lti:ServiceProvider
      lti:Vendor
      lti:ServiceOwner
    )
  ] ;
  rdfs:range xsd:dateTime ;
  rdfs:comment "A timestamp for the ServiceProvider record. This value is useful for determining which record is most current." .

lti:service_provider_name rdf:type owl:FunctionalProperty ;
  rdfs:domain lti:ServiceProvider ;
  rdfs:range lti:LocalizedName ;
  rdfs:comment "The name of the service provider, suitable for display to end users." .

lti:description rdf:type owl:FunctionalProperty ;
  rdfs:domain  [
    rdf:type owl:Class ;
    owl:unionOf (
      lti:ServiceProvider
      lti:ProductInfo
      lti:ResourceHandler
      lti:Vendor
      lti:ServiceOwner
    )
  ] ;
  rdfs:range lti:LocalizedText ;
  rdfs:comment "A description of the service provider, suitable for display to end-users." .

lti:support rdf:type owl:FunctionalProperty ;
  rdfs:domain  [
    rdf:type owl:Class ;
    owl:unionOf (
      lti:ServiceProvider
      lti:ProductInstance
    )
  ] ;
  rdfs:range lti:Contact ;
  rdfs:comment "Contact information for support from a service provider." .

lti:key rdf:type owl:FunctionalProperty ;
  rdfs:domain  [
    rdf:type owl:Class ;
    owl:unionOf (
      lti:IconInfo
      lti:LocalizedName
      lti:LocalizedText
      lti:ShortLocalizedName
    )
  ] ;
  rdfs:range lti-type:Name.Type ;
  rdfs:comment "If localization is supported then the 'key' attribute identifies a property in the resource bundle provided in response to the get-bundle-request message. The value of that property is the locale-specific path to the icon." .

lti:default_location rdf:type owl:FunctionalProperty ;
  rdfs:domain lti:IconInfo ;
  rdfs:range lti:IconEndpoint ;
  rdfs:comment "Specifies the default path to an icon.  The absolute URL is formed by appending this path to the appropriate base URL for icons." .

lti:icon_style rdf:type rdf:Property ;
  rdfs:domain lti:IconInfo ;
  rdfs:range lti:IconStyle ;
  rdfs:comment "The style of the icon referenced by this IconInfo." .

lti:default_value rdf:type owl:FunctionalProperty ;
  rdfs:domain  [
    rdf:type owl:Class ;
    owl:unionOf (
      lti:LocalizedName
      lti:LocalizedText
      lti:ShortLocalizedName
    )
  ] ;
  rdfs:range  [
    rdf:type owl:Class ;
    owl:unionOf (
      lti-type:LongName.Type
      lti-type:Text.Type
      lti-type:ShortName.Type
    )
  ] ;
  rdfs:comment "The default value for the display name.  This value is used if (1) the key attribute is undefined, (2) the localization capability is not enabled, or (3) a value for the specified key is not found in the locale-specific resource bundle." .

lti:enabled_capability rdf:type rdf:Property ;
  rdfs:domain  [
    rdf:type owl:Class ;
    owl:unionOf (
      lti:MessageHandler
      lti:ToolProxy
    )
  ] ;
  rdfs:range lti:Capability ;
  rdfs:comment "A capability that is enabled for messages handled by this MessageHandler." .

lti:message_type rdf:type owl:FunctionalProperty ;
  rdfs:domain lti:MessageHandler ;
  rdfs:range lti:MessageType ;
  rdfs:comment "The type of message that can be submitted to the Message Handler." .

lti:parameter rdf:type rdf:Property ;
  rdfs:domain lti:MessageHandler ;
  rdfs:range lti:Parameter ;
  rdfs:comment "Specifies a custom parameter that is expected by the MessageHandler." .

lti:product_name rdf:type owl:FunctionalProperty ;
  rdfs:domain lti:ProductInfo ;
  rdfs:range lti:LocalizedName ;
  rdfs:comment "A name for the product, suitable for display to end users." .

lti:product_version rdf:type owl:FunctionalProperty ;
  rdfs:domain lti:ProductInfo ;
  rdfs:range xsd:normalizedString ;
  rdfs:comment "This is the version of the product. " .

lti:technical_description rdf:type owl:FunctionalProperty ;
  rdfs:domain lti:ProductInfo ;
  rdfs:range lti:LocalizedText ;
  rdfs:comment "This is a human readable description of the technical aspects of this product that might be of interest to developers who wish to integrate with this product via LTI." .

lti:product_family rdf:type owl:FunctionalProperty ;
  rdfs:domain lti:ProductInfo ;
  rdfs:range lti:ProductFamily ;
  owl:inverseOf lti:version ;
  rdfs:comment "An inverse attribute that references the ProductFamily within which this ProductInfo is defined." .

lti:instance rdf:type rdf:Property ;
  rdfs:domain lti:ProductInfo ;
  rdfs:range lti:ProductInstance ;
  owl:inverseOf lti:product_info ;
  rdfs:comment "A deployed instance of a particular version of a product (Tool or Tool Consumer)." .

lti:vendor rdf:type owl:FunctionalProperty ;
  rdfs:domain lti:ProductFamily ;
  rdfs:range lti:Vendor ;
  owl:inverseOf lti:product ;
  rdfs:comment "The vendor that owns the ProductFamily." .

lti:version rdf:type rdf:Property ;
  rdfs:domain lti:ProductFamily ;
  rdfs:range lti:ProductInfo ;
  owl:inverseOf lti:product_family ;
  rdfs:comment "Encapsulates information about one version of the product." .

lti:lti_version rdf:type owl:FunctionalProperty ;
  rdfs:domain  [
    rdf:type owl:Class ;
    owl:unionOf (
      lti:ProductProfile
      lti:ToolProxy
    )
  ] ;
  rdfs:range  [
    rdf:type owl:Class ;
    owl:unionOf (
      xsd:normalizedString
      xsd:token
    )
  ] ;
  rdfs:comment "The identifier for an LTI version that the version supports.  A given product (Tool or Tool Consumer) may support multiple versions, but only one version is selected for use in the integration contract." .

lti:service_offered rdf:type rdf:Property ;
  rdfs:domain lti:ProductProfile ;
  rdfs:range lti:ServiceDescriptor ;
  rdfs:comment "The descriptor for a service offered by the product (Tool or Tool Consumer)." .

lti:product_instance rdf:type owl:FunctionalProperty ;
  rdfs:domain lti:ProductProfile ;
  rdfs:range lti:ProductInstance ;
  owl:inverseOf lti:profile ;
  rdfs:comment "An inverse attribute which references the ProductInstance within which this ProductProfile is defined." .

lti:capability_offered rdf:type rdf:Property ;
  rdfs:domain lti:ToolConsumerProfile ;
  rdfs:range lti:Capability ;
  rdfs:comment "A capability offered by the Tool Consumer to its integration partners." .

lti:message rdf:type rdf:Property ;
  rdfs:domain  [
    rdf:type owl:Class ;
    owl:unionOf (
      lti:ToolProfile
      lti:ResourceHandler
    )
  ] ;
  rdfs:range lti:MessageHandler ;
  rdfs:comment "A definition of a message supported by the resource handler." .

lti:resource_handler rdf:type rdf:Property ;
  rdfs:domain lti:ToolProfile ;
  rdfs:range lti:ResourceHandler ;
  rdfs:comment "A definition of a resource offered by the tool provider." .

lti:base_url_choice rdf:type rdf:Property ;
  rdfs:domain lti:ToolProfile ;
  rdfs:range lti:BaseUrlChoice ;
  rdfs:comment "Base URLs to use as a prefix to any incomplete URLs specified in the diocument." .

lti:resource_name rdf:type owl:FunctionalProperty ;
  rdfs:domain lti:ResourceHandler ;
  rdfs:range lti:LocalizedName ;
  rdfs:comment "The name of the resource handler suitable for display in the TC user interface." .

lti:resource_type rdf:type owl:FunctionalProperty ;
  rdfs:domain lti:ResourceHandler ;
  rdfs:range lti:ResourceType ;
  rdfs:comment "Identifies the type of resource associated with this ResourceHandler.  Resource types are identified by a code that is unique within a given ProductFamily." .

lti:icon_info rdf:type rdf:Property ;
  rdfs:domain lti:ResourceHandler ;
  rdfs:range lti:IconInfo ;
  rdfs:comment "Provides information about a graphical icon that represents the resource described by this ResourceHandler." .

lti:name rdf:type owl:FunctionalProperty ;
  rdfs:domain lti:Parameter ;
  rdfs:range xsd:Name ;
  rdfs:comment "The name of the parameter." .

lti:fixed rdf:type owl:FunctionalProperty ;
  rdfs:domain lti:Parameter ;
  rdfs:range lti-type:DataValue.Type ;
  rdfs:comment "Denotes that the value of the parameter is fixed at the time of definition within the product profile.  This value must be passed in each message of the associated message type." .

lti:variable rdf:type owl:FunctionalProperty ;
  rdfs:domain lti:Parameter ;
  rdfs:range lti-type:VariableName.Type ;
  rdfs:comment "Denotes that the parameter has a variable value that is automatically substituted at run-time.  The value of this attribute is the name for a variable whose value will be added to the message at run-time. " .

lti:vendor_name rdf:type owl:FunctionalProperty ;
  rdfs:domain lti:Vendor ;
  rdfs:range lti:LocalizedName ;
  rdfs:comment "Defines a human readable name for the Vendor.  The name should be suitable for display in management screens within the Tool Provider system." .

lti:website rdf:type owl:FunctionalProperty ;
  rdfs:domain lti:Vendor ;
  rdfs:range xsd:anyURI ;
  rdfs:comment "This is the URL of the vendor." .

lti:product rdf:type rdf:Property ;
  rdfs:domain lti:Vendor ;
  rdfs:range lti:ProductFamily ;
  owl:inverseOf lti:vendor ;
  rdfs:comment """<p>A group of related products offered by the Vendor.  All of the products within a given product family are different <em>versions</em> of the same product. </p>
<p>A vendor may have multiple product families.  For example, the same vendor might offer a discussion forum tool and also a white board tool.  Each of these tools corresponds to a different product family.</p>""" .

lti:contact rdf:type owl:FunctionalProperty ;
  rdfs:domain lti:Vendor ;
  rdfs:range lti:Contact ;
  rdfs:comment "Contact information for this Vendor." .

lti:absolute_path_allowed rdf:type owl:FunctionalProperty ;
  rdfs:domain lti:MessageType ;
  rdfs:range xsd:boolean ;
  rdfs:comment "Specifies whether the path for this message type is allowed to be specified using an absolute path.  A value of \"false\" means that the MessageHandler must declare a relative path." .

lti:message_class rdf:type owl:FunctionalProperty ;
  rdfs:domain lti:MessageType ;
  rdfs:range owl:Class ;
  rdfs:comment "This attribute identifies the formal Class definition the type of message that can be delivered to a given MessageHandler." .

lti:http_method rdf:type rdf:Property ;
  rdfs:domain lti:MessageType ;
  rdfs:range lti:HttpMethod ;
  rdfs:comment "Specifies an HTTP method (POST, GET, PUT, etc.) for the type of messages represented by this MessageType." .

lti:shared_secret rdf:type owl:FunctionalProperty ;
  rdfs:domain lti:SecurityContract ;
  rdfs:range xsd:string ;
  rdfs:comment """This is the shared secret used for communications between the Tool Consumer and the Tool Provider.  It is expected that the Tool Consumer present an interface to the administrative user for them to activate the Tool Proxy before this secret is ever used by the Tool Consumer. 
The shared secret may be updated when a tool is re-registered (see the reregisterTool operation of the ToolRegistrationService).  In addition, the TC and TP should provide interfaces which allow their respective administrators to change the shared secret through an out-of-band agreement.""" .

lti:tool_service rdf:type rdf:Property ;
  rdfs:domain lti:SecurityContract ;
  rdfs:range lti:ServiceProfile ;
  rdfs:comment "The profile for a Tool Consumer service that may be invoked by the Tool acting on its own (as opposed to acting as an agent for some end user).  " .

lti:end_user_service rdf:type rdf:Property ;
  rdfs:domain lti:SecurityContract ;
  rdfs:range lti:ServiceProfile ;
  rdfs:comment "The profile for a Tool Consumer service that may be invoked by the Tool when acting as an agent for some end user.  " .

lti:service rdf:type owl:FunctionalProperty ;
  rdfs:domain lti:ServiceProfile ;
  rdfs:range lti:ServiceDescriptor ;
  rdfs:comment "The descriptor for the service that is being profiled." .

lti:action rdf:type rdf:Property ;
  rdfs:domain  [
    rdf:type owl:Class ;
    owl:unionOf (
      lti:RestServiceProfile
      lti:RestService
    )
  ] ;
  rdfs:range lti:HttpMethod ;
  rdfs:comment "Specifies an HTTP method (POST, GET, PUT, etc.) which the integration partner intends to use.   A RestServiceProfile may include more than one action.  However, the set of actions declared in a RestServiceProfile must be a subset of actions declared in the RestService referenced by the <code>service</code> property." .

lti:resource_type_owner rdf:type owl:FunctionalProperty ;
  rdfs:domain lti:ResourceType ;
  rdfs:range lti:ProductFamily .

lti:code rdf:type owl:FunctionalProperty ;
  rdfs:domain lti:HasCode ;
  rdfs:range lti-type:Token.Type ;
  rdfs:comment "A unique identifier for the resource." .

lti:format rdf:type rdf:Property ;
  rdfs:domain lti:RestService ;
  rdfs:range xsd:normalizedString ;
  rdfs:comment "The content type (also known as media type) of resources accessed via the endpoint defined by this RestService descriptor.   The endpoint of a REST service may support more than one content type if content negotiation is enabled as described in the <a href=\"http://www.w3.org/Protocols/rfc2616/rfc2616-sec12.html\">HTTP 1.1</a> specification." .

lti:endpoint rdf:type owl:FunctionalProperty ;
  rdfs:domain lti:RestService ;
  rdfs:range xsd:anyURI ;
  rdfs:comment "A URI template that defines the REST endpoint for resources that may be accessed via the REST service.  The URI template should conform to the syntax in the proposed IETF standard [<a href=\"http://www.ietf.org/id/draft-gregorio-uritemplate-08.txt\">draft-gregorio-uritemplate-08</a>]. " .

lti:service_provider rdf:type owl:FunctionalProperty ;
  rdfs:domain lti:ProductInstance ;
  rdfs:range lti:ServiceProvider ;
  rdfs:comment "This is the service provider that hosts the deployed product." .

lti:product_info rdf:type owl:FunctionalProperty ;
  rdfs:domain lti:ProductInstance ;
  rdfs:range lti:ProductInfo ;
  owl:inverseOf lti:instance ;
  rdfs:comment "This is metadata about the product described in the profile." .

lti:profile rdf:type rdf:Property ;
  rdfs:domain lti:ProductInstance ;
  rdfs:range lti:ProductProfile ;
  owl:inverseOf lti:product_instance ;
  rdfs:comment "A resource that presents a view of this ProductInstance to one or more integration partners." .

lti:service_owner rdf:type owl:FunctionalProperty ;
  rdfs:domain lti:ProductInstance ;
  rdfs:range lti:ServiceOwner ;
  rdfs:comment "The entity that owns the services provided by this product instance." .

lti:service_owner_name rdf:type owl:FunctionalProperty ;
  rdfs:domain lti:ServiceOwner ;
  rdfs:range lti:LocalizedName ;
  rdfs:comment "The name of the service owner, suitable for display to end users. " .

lti:tool_proxy_guid rdf:type owl:FunctionalProperty ;
  rdfs:domain lti:ToolProxy ;
  rdfs:range lti-type:GUID.Type ;
  rdfs:comment "The globally unique identifier for the ToolProxy (a.k.a. integration contract)." .

lti:tool_profile rdf:type owl:FunctionalProperty ;
  rdfs:domain lti:ToolProxy ;
  rdfs:range lti:ToolProfile ;
  rdfs:comment "The profile of the Tool that is participating in the integration governed by this ToolProxy." .

lti:security_contract rdf:type owl:FunctionalProperty ;
  rdfs:domain lti:ToolProxy ;
  rdfs:range lti:SecurityContract ;
  rdfs:comment "The security aspect of an integration contract between two parties." .

lti:tool_consumer_profile rdf:type owl:FunctionalProperty ;
  rdfs:domain lti:ToolProxy ;
  rdfs:range lti:ToolConsumerProfile ;
  rdfs:comment "The profile of the Tool Consumer that is participating in the integration governed by this ToolProxy." .

lti:context rdf:type owl:FunctionalProperty ;
  rdfs:domain lti:ToolProxyBinding ;
  rdfs:range lti:Context ;
  rdfs:comment "The learning Context associated with this <code>ToolProxyBinding</code>." .

lti:resourceLinkId rdf:type owl:FunctionalProperty ;
  rdfs:domain lti:ResourceLink ;
  rdfs:range lti-type:GUID.Type ;
  rdfs:comment "A globally unique identifier for this LTI link." .

lti:contextId rdf:type owl:FunctionalProperty ;
  rdfs:domain lti:Context ;
  rdfs:range xsd:normalizedString ;
  rdfs:comment "A unique string provided by the tool consumer to identify the context (as passed in the context_id launch parameter)." .

lti:sourcedId rdf:type owl:FunctionalProperty ;
  rdfs:domain lti:Context ;
  rdfs:range xsd:normalizedString ;
  rdfs:comment "A unique identifier for the context as provisioned by an external system such as an SIS." .

lti:lineItem rdf:type rdf:Property ;
  rdfs:domain lti:Context ;
  rdfs:range liso:LineItem ;
  owl:inverseOf liso:lineItemOf ;
  rdfs:comment "A LineItem that records results for some learning activity within this context." .

lti:lineItems rdf:type owl:FunctionalProperty ;
  rdfs:domain lti:Context ;
  rdfs:range liso:LineItemContainer ;
  rdfs:comment """The container that holds the collection of LineItem resources for this Context.  In general, this container is optional.  However, if the Context has any associated LineItems, then the container is required.  As a best practice, implementations every Context should expose a LineItemContainer to clients, even if it is empty.
""" .

lti:custom rdf:type owl:FunctionalProperty ;
  rdfs:domain lti:ToolSettingsContainer ;
  rdfs:range lti:PropertyMap ;
  rdfs:comment "A collection of custom properties defined by the Tool Provider and stored in this ToolSettingsContainer." .

lti:settingsResourceLink rdf:type owl:FunctionalProperty ;
  rdfs:domain lti:LtiLink ;
  rdfs:range lti:ResourceLink ;
  rdfs:comment "The resource link associated with the settings." .

lti:frame rdf:type lti:DocumentTarget .

lti:embed rdf:type lti:DocumentTarget .

lti:iframe rdf:type lti:DocumentTarget .

lti:window rdf:type lti:DocumentTarget .

lti:popup rdf:type lti:DocumentTarget .

lti:overlay rdf:type lti:DocumentTarget .

lti:none rdf:type lti:DocumentTarget .
@prefix rdf: <http://www.w3.org/1999/02/22-rdf-syntax-ns#> .
@prefix rdfs: <http://www.w3.org/2000/01/rdf-schema#> .
@prefix bind: <http://purl.org/semantictools/v1/vocab/bind#> .
@prefix lti: <http://ld.kinexis.com/vocab/lti/v2/lti#> .

lti:BaseUrlChoice rdf:type bind:EmbeddableClass .
lti:BaseUrlChoice rdfs:subClassOf
  [ rdf:type bind:AssociationQualifier ;
    bind:onProperty lti:selector ;
    bind:associationType bind:Composition
  ] .
lti:BaseUrlSelector rdf:type bind:EmbeddableClass .
lti:BaseUrlSelector rdfs:subClassOf
  [ rdf:type bind:AssociationQualifier ;
    bind:onProperty lti:applies_to ;
    bind:associationType bind:Aggregation
  ] .
lti:Contact rdf:type bind:EmbeddableClass .
lti:Endpoint rdf:type bind:EmbeddableClass .
lti:Endpoint rdf:type bind:AbstractClass .
lti:ServiceProvider rdf:type bind:Addressable .
lti:ServiceProvider rdfs:subClassOf
  [ rdf:type bind:AssociationQualifier ;
    bind:onProperty lti:support ;
    bind:associationType bind:Composition
  ] .
lti:IconEndpoint rdf:type bind:EmbeddableClass .
lti:IconInfo rdf:type bind:EmbeddableClass .
lti:IconInfo rdfs:subClassOf
  [ rdf:type bind:AssociationQualifier ;
    bind:onProperty lti:default_location ;
    bind:associationType bind:Composition
  ], 
  [ rdf:type bind:AssociationQualifier ;
    bind:onProperty lti:icon_style ;
    bind:associationType bind:Aggregation
  ] .
lti:IconStyle rdf:type bind:Enum .
lti:LocalizedName rdf:type bind:EmbeddableClass .
lti:LocalizedText rdf:type bind:EmbeddableClass .
lti:MessageHandler rdf:type bind:EmbeddableClass .
lti:MessageHandler rdfs:subClassOf
  [ rdf:type bind:AssociationQualifier ;
    bind:onProperty lti:enabled_capability ;
    bind:associationType bind:Aggregation
  ], 
  [ rdf:type bind:AssociationQualifier ;
    bind:onProperty lti:message_type ;
    bind:associationType bind:Aggregation
  ], 
  [ rdf:type bind:AssociationQualifier ;
    bind:onProperty lti:parameter ;
    bind:associationType bind:Composition
  ] .
lti:ProductInfo rdf:type bind:EmbeddableClass .
lti:ProductInfo rdfs:subClassOf
  [ rdf:type bind:AssociationQualifier ;
    bind:onProperty lti:instance ;
    bind:associationType bind:Composition
  ] .
lti:ProductFamily rdf:type bind:EmbeddableClass .
lti:ProductFamily rdfs:subClassOf
  [ rdf:type bind:AssociationQualifier ;
    bind:onProperty lti:version ;
    bind:associationType bind:Composition
  ] .
lti:ProductProfile rdf:type bind:Addressable .
lti:ProductProfile rdf:type bind:AbstractClass .
lti:ProductProfile rdfs:subClassOf
  [ rdf:type bind:AssociationQualifier ;
    bind:onProperty lti:service_offered ;
    bind:associationType bind:Composition
  ] .
lti:ServiceDescriptor rdf:type bind:Addressable .
lti:ServiceDescriptor rdf:type bind:AbstractClass .
lti:ToolConsumerProfile rdf:type bind:Addressable .
lti:ToolConsumerProfile rdfs:subClassOf
  [ rdf:type bind:AssociationQualifier ;
    bind:onProperty lti:capability_offered ;
    bind:associationType bind:Aggregation
  ] .
lti:ToolProfile rdf:type bind:Addressable .
lti:ToolProfile rdfs:subClassOf
  [ rdf:type bind:AssociationQualifier ;
    bind:onProperty lti:message ;
    bind:associationType bind:Composition
  ], 
  [ rdf:type bind:AssociationQualifier ;
    bind:onProperty lti:resource_handler ;
    bind:associationType bind:Composition
  ], 
  [ rdf:type bind:AssociationQualifier ;
    bind:onProperty lti:base_url_choice ;
    bind:associationType bind:Composition
  ] .
lti:ResourceHandler rdf:type bind:EmbeddableClass .
lti:ResourceHandler rdfs:subClassOf
  [ rdf:type bind:AssociationQualifier ;
    bind:onProperty lti:resource_type ;
    bind:associationType bind:Aggregation
  ], 
  [ rdf:type bind:AssociationQualifier ;
    bind:onProperty lti:message ;
    bind:associationType bind:Composition
  ], 
  [ rdf:type bind:AssociationQualifier ;
    bind:onProperty lti:icon_info ;
    bind:associationType bind:Composition
  ] .
lti:Parameter rdf:type bind:EmbeddableClass .
lti:ShortLocalizedName rdf:type bind:EmbeddableClass .
lti:Vendor rdf:type bind:Addressable .
lti:Vendor rdfs:subClassOf
  [ rdf:type bind:AssociationQualifier ;
    bind:onProperty lti:product ;
    bind:associationType bind:Composition
  ], 
  [ rdf:type bind:AssociationQualifier ;
    bind:onProperty lti:contact ;
    bind:associationType bind:Composition
  ] .
lti:Capability rdf:type bind:Enum .
lti:MessageType rdf:type bind:EmbeddableClass .
lti:MessageType rdfs:subClassOf
  [ rdf:type bind:AssociationQualifier ;
    bind:onProperty lti:http_method ;
    bind:associationType bind:Composition
  ] .
lti:SecurityContract rdf:type bind:EmbeddableClass .
lti:SecurityContract rdfs:subClassOf
  [ rdf:type bind:AssociationQualifier ;
    bind:onProperty lti:tool_service ;
    bind:associationType bind:Composition
  ], 
  [ rdf:type bind:AssociationQualifier ;
    bind:onProperty lti:end_user_service ;
    bind:associationType bind:Composition
  ] .
lti:ServiceProfile rdf:type bind:EmbeddableClass .
lti:ServiceProfile rdf:type bind:AbstractClass .
lti:ServiceProfile rdfs:subClassOf
  [ rdf:type bind:AssociationQualifier ;
    bind:onProperty lti:service ;
    bind:associationType bind:Aggregation
  ] .
lti:RestServiceProfile rdfs:subClassOf
  [ rdf:type bind:AssociationQualifier ;
    bind:onProperty lti:action ;
    bind:associationType bind:Aggregation
  ] .
lti:ResourceType rdf:type bind:EmbeddableClass .
lti:ResourceType rdfs:subClassOf
  [ rdf:type bind:AssociationQualifier ;
    bind:onProperty lti:resource_type_owner ;
    bind:inverseAssociationType bind:Composition ;
    bind:inverseUnboundedCardinality true
  ] .
lti:HasCode rdf:type bind:AbstractClass .
lti:RestService rdf:type bind:Addressable .
lti:RestService rdfs:subClassOf
  [ rdf:type bind:AssociationQualifier ;
    bind:onProperty lti:action ;
    bind:associationType bind:Aggregation
  ] .
lti:ProductInstance rdfs:subClassOf
  [ rdf:type bind:AssociationQualifier ;
    bind:onProperty lti:service_provider ;
    bind:associationType bind:Aggregation ;
    bind:inverseUnboundedCardinality true
  ], 
  [ rdf:type bind:AssociationQualifier ;
    bind:onProperty lti:profile ;
    bind:associationType bind:Composition
  ], 
  [ rdf:type bind:AssociationQualifier ;
    bind:onProperty lti:support ;
    bind:associationType bind:Composition
  ], 
  [ rdf:type bind:AssociationQualifier ;
    bind:onProperty lti:service_owner ;
    bind:associationType bind:Aggregation
  ] .
lti:ToolProxy rdf:type bind:Addressable .
lti:ToolProxy rdfs:subClassOf
  [ rdf:type bind:AssociationQualifier ;
    bind:onProperty lti:tool_profile ;
    bind:associationType bind:Aggregation
  ], 
  [ rdf:type bind:AssociationQualifier ;
    bind:onProperty lti:security_contract ;
    bind:associationType bind:Composition
  ], 
  [ rdf:type bind:AssociationQualifier ;
    bind:onProperty lti:tool_consumer_profile ;
    bind:associationType bind:Aggregation
  ], 
  [ rdf:type bind:AssociationQualifier ;
    bind:onProperty lti:enabled_capability ;
    bind:associationType bind:Aggregation
  ] .
lti:ToolProxyBinding rdf:type bind:Addressable .
lti:ToolProxyBinding rdfs:subClassOf
  [ rdf:type bind:AssociationQualifier ;
    bind:onProperty lti:context ;
    bind:associationType bind:Aggregation
  ] .
lti:ResourceLink rdf:type bind:Addressable .
lti:Context rdf:type bind:Addressable .
lti:Context rdfs:subClassOf
  [ rdf:type bind:AssociationQualifier ;
    bind:onProperty lti:lineItem ;
    bind:associationType bind:Composition
  ], 
  [ rdf:type bind:AssociationQualifier ;
    bind:onProperty lti:lineItems ;
    bind:associationType bind:Composition
  ] .
lti:ToolSettingsContainer rdfs:subClassOf
  [ rdf:type bind:AssociationQualifier ;
    bind:onProperty lti:custom ;
    bind:associationType bind:Composition
  ] .
lti:LtiLink rdf:type bind:Addressable .
lti:LtiLink rdfs:subClassOf
  [ rdf:type bind:AssociationQualifier ;
    bind:onProperty lti:settingsResourceLink ;
    bind:associationType bind:Aggregation
  ] .
lti:DocumentTarget rdf:type bind:Enum .

lti:HttpMethod rdf:type bind:Enum .
@prefix ltiv: <http://ld.kinexis.com/vocab/lti/v2/variable#> .
@prefix lti: <http://ld.kinexis.com/vocab/lti/v2/lti#> .
@prefix owl: <http://www.w3.org/2002/07/owl#> .
@prefix rdf: <http://www.w3.org/1999/02/22-rdf-syntax-ns#> .
@prefix rdfs: <http://www.w3.org/2000/01/rdf-schema#> .
@prefix xsd: <http://www.w3.org/2001/XMLSchema#> .
@prefix bind: <http://purl.org/semantictools/v1/vocab/bind#> .

<http://ld.kinexis.com/vocab/lti/v2/variable#> a owl:Ontology  ;
  rdfs:label "LTI Variables" ;
  a bind:TargetNamespace ;
  bind:suggestedPrefix "ltiv" .

ltiv:Variable rdf:type owl:Class ;
  rdfs:subClassOf lti:Capability ; 
  rdfs:comment "Custom parameter substitution variables." .

ltiv:User.id rdf:type ltiv:Variable ;
  rdfs:comment "Corresponds to the user_id launch parameterfrom the <code>LaunchMixin</code> class.  This is the local identifier for the user within the Tool Consumer system." .

ltiv:User.image rdf:type ltiv:Variable ;
  rdfs:comment "The URL for an image of the user suitable for use as a profile picture or avatar." .

ltiv:Person.sourcedId rdf:type ltiv:Variable ;
  rdfs:comment """The LIS identifier for the user.  
<p>In the LIS Database, this value corresponds to <code>personRecord/sourcedId</code></p>""" .

ltiv:Person.name.full rdf:type ltiv:Variable ;
  rdfs:comment """The full name of the user.
<p>In the LIS Database, this value corresponds to 
<pre>personRecord/person/formname/[formnameType/instanceValue/text=\"Full\"] /formattedName/text
</pre></p>""" .

ltiv:Person.name.family rdf:type ltiv:Variable ;
  rdfs:comment """The family name of the user.
<p>In the LIS Database, this value corresponds to 
<pre>personRecord/person/name/partName[instanceName/text=\"Family\u201d]/instanceValue/text 
</pre></p>""" .

ltiv:Person.name.given rdf:type ltiv:Variable ;
  rdfs:comment """The given name of the user.
<p>In the LIS Database, this value corresponds to 
<pre>personRecord/person/name/partName[instanceName/text=\"Given\u201d]/instanceValue/text
</pre></p>""" .

ltiv:Person.name.middle rdf:type ltiv:Variable ;
  rdfs:comment """The middle name of the user.
<p>In the LIS Database, this value corresponds to 
<pre>personRecord/person/name/partName[instanceName/text=\"Middle\u201d]/instanceValue/text 
</pre></p>""" .

ltiv:Person.name.prefix rdf:type ltiv:Variable ;
  rdfs:comment """The prefix for the user's name, such as <em>Dr.</em>, <em>Mr.</em>, <em>Ms.</em> etc.
<p>In the LIS Database, this value corresponds to 
<pre>personRecord/person/name/partName[instanceName/text=\"Prefix\u201d]/instanceValue/text 
</pre></p>""" .

ltiv:Person.name.suffix rdf:type ltiv:Variable ;
  rdfs:comment """The suffix for the user's name, such as <em>Jr.</em>, <em>II</em>,  etc.
<p>In the LIS Database, this value corresponds to 
<pre>personRecord/person/name/partName[instanceName/text=\"Suffix\u201d]/instanceValue/text 
</pre></p>""" .

ltiv:Person.address.street1 rdf:type ltiv:Variable ;
  rdfs:comment """The first line of the user's street address.
<p>In the LIS Database, this value corresponds to 
<pre>personRecord/person/address/[addressType/instanceValue/text=\"Preferred\"]addressPart /nameValuePair /[instanceName/text=\"NonFieldedStreetAddress1\"]/instanceValue /text  
</pre></p>""" .

ltiv:Person.address.street2 rdf:type ltiv:Variable ;
  rdfs:comment """The second line of the user's street address.
<p>In the LIS Database, this value corresponds to 
<pre>personRecord/person/address/[addressType/instanceValue/text=\"Preferred\"]  addressPart /nameValuePair[instanceName/text=\"NonFieldedStreetAddress2\"] /instanceValue/text 
</pre></p>""" .

ltiv:Person.address.street3 rdf:type ltiv:Variable ;
  rdfs:comment """The third line of the user's street address.
<p>In the LIS Database, this value corresponds to 
<pre>personRecord/person/address/[addressType/instanceValue/text=\"Preferred\"]addressPart /nameValuePair /[instanceName/text=\"NonFieldedStreetAddress3\"] /instanceValue/text
</pre></p>""" .

ltiv:Person.address.street4 rdf:type ltiv:Variable ;
  rdfs:comment """The fourth line of the user's street address.
<p>In the LIS Database, this value corresponds to 
<pre>personRecord/person/address/[addressType/instanceValue/text=\"Preferred\"]addressPart /nameValuePair /[instanceName/text=\"NonFieldedStreetAddress4\"] /instanceValue/text
</pre></p>""" .

ltiv:Person.address.locality rdf:type ltiv:Variable ;
  rdfs:comment """The city, town, or other locality within the user's address.
<p>In the LIS Database, this value corresponds to 
<pre>personRecord/person/address/[addressType/instanceValue/text=\"Preferred\"]addressPart /nameValuePair /[instanceName/text=\"Locality\"]/instanceValue/text
</pre></p>""" .

ltiv:Person.address.statepr rdf:type ltiv:Variable ;
  rdfs:comment """The state or province within the user's address.
<p>In the LIS Database, this value corresponds to 
<pre>personRecord/person/address/[addressType/instanceValue/text=\"Preferred\"]addressPart /nameValuePair/[instanceName/text=\"Statepr\"]/instanceValue/text
</pre></p>""" .

ltiv:Person.address.country rdf:type ltiv:Variable ;
  rdfs:comment """The country within the user's address.
<p>In the LIS Database, this value corresponds to 
<pre>personRecord/person/address/[addressType/instanceValue/text=\"Preferred\"]addressPart /nameValuePair /[instanceName/text=\"Country\"]/instanceValue/text
</pre></p>""" .

ltiv:Person.address.postcode rdf:type ltiv:Variable ;
  rdfs:comment """The postal code within the user's address.
<p>In the LIS Database, this value corresponds to 
<pre>personRecord/person/address/[addressType/instanceValue/text=\"Preferred\"]addressPart /nameValuePair /[instanceName/text=\"Postcode\"]/instanceValue/text
</pre></p>""" .

ltiv:Person.address.timezone rdf:type ltiv:Variable ;
  rdfs:comment """The user's time zone.
<p>In the LIS Database, this value corresponds to 
<pre>personRecord/person/address/[addressType/instanceValue/text=\"Preferred\"]addressPart /nameValuePair /[instanceName/text=\"Timezone\"]/instanceValue/text
</pre></p>""" .

ltiv:Person.phone.mobile rdf:type ltiv:Variable ;
  rdfs:comment """The user's mobile phone number
<p>In the LIS Database, this value corresponds to 
<pre>personRecord/person/contactinfo[contactinfoType/instanceValue/text=\"Mobile\"] /contactInfoValue/text
</pre></p>""" .

ltiv:Person.phone.primary rdf:type ltiv:Variable ;
  rdfs:comment """The user's primary phone number
<p>In the LIS Database, this value corresponds to 
<pre>personRecord/person/contactinfo [contactinfoType/instanceValue/text=\"Telephone_Primary\"]/contactinfoValue /text
</pre></p>""" .

ltiv:Person.phone.home rdf:type ltiv:Variable ;
  rdfs:comment """The user's home phone number
<p>In the LIS Database, this value corresponds to 
<pre>personRecord/person/contactinfo [contactinfoType/instanceValue/text=\"Telephone_Home\"]/contactinfoValue /text
</pre></p>""" .

ltiv:Person.phone.work rdf:type ltiv:Variable ;
  rdfs:comment """The user's work phone number.
<p>In the LIS Database, this value corresponds to 
<pre>personRecord/person/contactinfo [contactinfoType/instanceValue/text=\"Telephone_Work\"]/contactinfoValue /text
</pre></p>""" .

ltiv:Person.email.primary rdf:type ltiv:Variable ;
  rdfs:comment """The user's primary email address.
<p>In the LIS Database, this value corresponds to 
<pre>personRecord/person/contactinfo[contactinfoType/instanceValue/text=\"Email_Primary\"] /contactinfoValue/text
</pre></p>""" .

ltiv:Person.email.personal rdf:type ltiv:Variable ;
  rdfs:comment """The user's personal email address
<p>In the LIS Database, this value corresponds to 
<pre>person/contactinfo[contactinfoType/instanceValue/text=\"Email_Personal\"]/contactinfoValue /text
</pre></p>""" .

ltiv:Person.webaddress rdf:type ltiv:Variable ;
  rdfs:comment """The user's web address.  This could be a facebook address, a blog, or any other web address linked to the user.  The value should be a URL.
<p>In the LIS Database, this value corresponds to 
<pre>personRecord/person/contactinfo[contactinfoType/instanceValue/text=\"Web-Address\"] /contactinfoValue/text
</pre></p>""" .

ltiv:Person.sms rdf:type ltiv:Variable ;
  rdfs:comment """The number at which the user prefers to receive SMS text messages.
<p>In the LIS Database, this value corresponds to 
<pre>personRecord/person/contactinfo[contactinfoType/instanceValue/text=\"SMS\"]  /contactinfoValue/text
</pre></p>""" .

ltiv:CourseTemplate.sourcedId rdf:type ltiv:Variable ;
  rdfs:comment """The LIS identifier for the Course Template.
<p>In the LIS Database, this value corresponds to 
<pre>courseTemplateRecord/sourcedId
</pre></p>""" .

ltiv:CourseTemplate.label rdf:type ltiv:Variable ;
  rdfs:comment """A human readable label used to help identify the Course Template.
<p>In the LIS Database, this value corresponds to 
<pre>courseTemplateRecord/courseTemplate/label/textString
</pre></p>""" .

ltiv:CourseTemplate.title rdf:type ltiv:Variable ;
  rdfs:comment """The title of the Course Template.
<p>In the LIS Database, this value corresponds to 
<pre>courseTemplateRecord/courseTemplate/title/textString
</pre></p>""" .

ltiv:CourseTemplate.shortDescription rdf:type ltiv:Variable ;
  rdfs:comment """A short description of the Course Template.
<p>In the LIS Database, this value corresponds to 
<pre>courseTemplateRecord/courseTemplate/catalogDescription/shortDescription
</pre></p>""" .

ltiv:CourseTemplate.longDescription rdf:type ltiv:Variable ;
  rdfs:comment """A long description of the Course Template.
<p>In the LIS Database, this value corresponds to 
<pre>courseTemplateRecord/courseTemplate/catalogDescription/longDescription
</pre></p>""" .

ltiv:CourseTemplate.courseNumber rdf:type ltiv:Variable ;
  rdfs:comment """The course number, such as \"Biology 101\".  In general, this number is not just a numeric value.
<p>In the LIS Database, this value corresponds to 
<pre>courseTemplateRecord/courseTemplate/courseNumber/textString
</pre></p>""" .

ltiv:CourseTemplate.credits rdf:type ltiv:Variable ;
  rdfs:comment """The default credits set for this Course Template.
<p>In the LIS Database, this value corresponds to 
<pre>courseTemplateRecord/courseTemplate/defaultCredits/textString
</pre></p>""" .

ltiv:CourseOffering.sourcedId rdf:type ltiv:Variable ;
  rdfs:comment """The LIS identifier for the Course Offering.
<p>In the LIS Database, this value corresponds to 
<pre>courseOfferingRecord/sourcedId
</pre></p>""" .

ltiv:CourseOffering.label rdf:type ltiv:Variable ;
  rdfs:comment """A human readable label for the Course Offering
<p>In the LIS Database, this value corresponds to 
<pre>courseOfferingRecord/courseOffering/label
</pre></p>""" .

ltiv:CourseOffering.title rdf:type ltiv:Variable ;
  rdfs:comment """The title of the Course Offering.
<p>In the LIS Database, this value corresponds to 
<pre>courseOfferingRecord/courseOffering/title
</pre></p>""" .

ltiv:CourseOffering.shortDescription rdf:type ltiv:Variable ;
  rdfs:comment """A short description of the Course Offering.
<p>In the LIS Database, this value corresponds to 
<pre>courseOfferingRecord/courseOffering/catalogDescription/shortDescription
</pre></p>""" .

ltiv:CourseOffering.longDescription rdf:type ltiv:Variable ;
  rdfs:comment """A long description of the Course Offering.
<p>In the LIS Database, this value corresponds to 
<pre>courseOfferingRecord/courseOffering/catalogDescription/longDescription
</pre></p>""" .

ltiv:CourseOffering.credits rdf:type ltiv:Variable ;
  rdfs:comment """The default credits set for this Course Offering
<p>In the LIS Database, this value corresponds to 
<pre>courseOfferingRecord/courseOffering/defaultCredits/textString
</pre></p>""" .

ltiv:CourseOffering.academicSession rdf:type ltiv:Variable ;
  rdfs:comment """The text data that is used to describe the academic session for the course offering.
<p>In the LIS Database, this value corresponds to 
<pre>courseOfferingRecord/courseOffering/defaultCredits/textString
</pre></p>""" .

ltiv:CourseSection.sourcedId rdf:type ltiv:Variable ;
  rdfs:comment """The LIS identifier for the Course Section
<p>In the LIS Database, this value corresponds to 
<pre>courseSection/sourcedId
</pre></p>""" .

ltiv:CourseSection.label rdf:type ltiv:Variable ;
  rdfs:comment """A human readable label for the Course Section.
<p>In the LIS Database, this value corresponds to 
<pre>courseSectionRecord/courseSection/label
</pre></p>""" .

ltiv:CourseSection.title rdf:type ltiv:Variable ;
  rdfs:comment """The title of the Course Section.
<p>In the LIS Database, this value corresponds to 
<pre>courseSectionRecord/courseSection/title
</pre></p>""" .

ltiv:CourseSection.shortDescription rdf:type ltiv:Variable ;
  rdfs:comment """A short description of the Course Section.
<p>In the LIS Database, this value corresponds to 
<pre>courseSectionRecord/courseSection/catalogDescription/shortDescription
</pre></p>""" .

ltiv:CourseSection.longDescription rdf:type ltiv:Variable ;
  rdfs:comment """A long description of the Course Section.
<p>In the LIS Database, this value corresponds to 
<pre>courseSectionRecord/courseSection/catalogDescription/longDescription
</pre></p>""" .

ltiv:CourseSection.courseNumber rdf:type ltiv:Variable ;
  rdfs:comment """The course number, such as \"Biology 101\".  In general, this number is not just a numeric value.
<p>In the LIS Database, this value corresponds to 
<pre>courseSectionRecord/courseSection/courseNumber/textString
</pre></p>""" .

ltiv:CourseSection.credits rdf:type ltiv:Variable ;
  rdfs:comment """The default credits set for the Course Section.
<p>In the LIS Database, this value corresponds to 
<pre>courseSectionRecord/courseSection/defaultCredits/textString
</pre></p>""" .

ltiv:CourseSection.maxNumberofStudents rdf:type ltiv:Variable ;
  rdfs:comment """The maximum number of students that can be enrolled in the Course Section.
<p>In the LIS Database, this value corresponds to 
<pre>courseSectionRecord/courseSection/maxNumberofStudents
</pre></p>""" .

ltiv:CourseSection.numberofStudents rdf:type ltiv:Variable ;
  rdfs:comment """The number of students who are enrolled in the Course Section.
<p>In the LIS Database, this value corresponds to 
<pre>courseSectionRecord/courseSection/numberofStudents
</pre></p>""" .

ltiv:CourseSection.dept rdf:type ltiv:Variable ;
  rdfs:comment """The department within which the Course Section is offered.
<p>In the LIS Database, this value corresponds to 
<pre>courseSectionRecord/courseSection/org[type/textString=\"Dept\"]/orgName/textString
</pre></p>""" .

ltiv:CourseSection.timeFrame.begin rdf:type ltiv:Variable ;
  rdfs:comment """The date and time when the Course Section becomes available.
<p>In the LIS Database, this value corresponds to 
<pre>courseSectionRecord/courseSection/timeFrame/begin
</pre></p>""" .

ltiv:CourseSection.timeFrame.end rdf:type ltiv:Variable ;
  rdfs:comment """The date and time after which the Course Section is no longer available.
<p>In the LIS Database, this value corresponds to 
<pre>courseSectionRecord/courseSection/timeFrame/end
</pre></p>""" .

ltiv:CourseSection.enrollControll.accept rdf:type ltiv:Variable ;
  rdfs:comment """A boolean value that specifies whether the Course Section is accepting enrollments.
<p>In the LIS Database, this value corresponds to 
<pre>courseSectionRecord/courseSection/enrollControl/enrollAccept
</pre></p>""" .

ltiv:CourseSection.enrollControl.allowed rdf:type ltiv:Variable ;
  rdfs:comment """A boolean value that specifies whether the Tool Provider can enroll people in the Course Section.  The value <code>false</code> indicates that only the source system can enroll people.
<p>In the LIS Database, this value corresponds to 
<pre>courseSectionRecord/courseSection/enrollControl/enrollAllowed
</pre></p>""" .

ltiv:CourseSection.dataSource rdf:type ltiv:Variable ;
  rdfs:comment """An identifier for the original source system of the CourseSection object.
<p>In the LIS Database, this value corresponds to 
<pre>courseSectionRecord/courseSection/dataSource
</pre></p>""" .

ltiv:CourseSection.sourceSectionId rdf:type ltiv:Variable ;
  rdfs:comment """The identifier for the source Course Section from which the target Course Section was cloned.
<p>In the LIS Database, this value corresponds to 
<pre>createCourseSectionFromCourseSectionRequest/sourcedId
</pre></p>""" .

ltiv:Group.sourcedId rdf:type ltiv:Variable ;
  rdfs:comment """The LIS identifier for the Group.
<p>In the LIS Database, this value corresponds to 
<pre>groupRecord/sourcedId
</pre></p>""" .

ltiv:Group.grouptype rdf:type ltiv:Variable ;
  rdfs:comment "A URI that uniquely identifies the type of group.  This convention differs from the LIS convention of using a structured object to describe the type of a group.  Ideally, the URI should resolve to JSON-LD document that describes the group type.  However, any URI that uniquely identifies the group type in accordance with the rules of the grouptype scheme is acceptable." .

ltiv:Group.email rdf:type ltiv:Variable ;
  rdfs:comment """An email address used for posting messages to members of the group.  
<p>In the LIS Database, this value corresponds to 
<pre>groupRecord/group/email
</pre></p>""" .

ltiv:Group.url rdf:type ltiv:Variable ;
  rdfs:comment """The web address of the Group.
<p>In the LIS Database, this value corresponds to 
<pre>groupRecord/group/url
</pre></p>""" .

ltiv:Group.timeFrame.begin rdf:type ltiv:Variable ;
  rdfs:comment """The date and time when access to Group resources begins.
<p>In the LIS Database, this value corresponds to 
<pre>groupRecord/group/timeframe/begin
</pre></p>""" .

ltiv:Group.timeFrame.end rdf:type ltiv:Variable ;
  rdfs:comment """The date and time when access to Group resources ends.
<p>In the LIS Database, this value corresponds to 
<pre>groupRecord/group/timeframe/end
</pre></p>""" .

ltiv:Group.enrollControl.accept rdf:type ltiv:Variable ;
  rdfs:comment """A boolean value that specifies whether the Group is accepting enrollments.
<p>In the LIS Database, this value corresponds to 
<pre>groupRecord/group/enrollControl/enrollAccept
</pre></p>""" .

ltiv:Group.enrollControl.allowed rdf:type ltiv:Variable ;
  rdfs:comment """A boolean value that specifies whether the Tool Provider can enroll people in the Group.  The value <code>false</code> indicates that only the source system can enroll people.
<p>In the LIS Database, this value corresponds to 
<pre>groupRecord/group/enrollControl/enrollAllowed
</pre></p>""" .

ltiv:Group.shortDescription rdf:type ltiv:Variable ;
  rdfs:comment """A short description of the Group.
<p>In the LIS Database, this value corresponds to 
<pre>groupRecord/group/description/shortDescription
</pre></p>""" .

ltiv:Group.longDescription rdf:type ltiv:Variable ;
  rdfs:comment """A long description of the Group.
<p>In the LIS Database, this value corresponds to 
<pre>groupRecord/group/description/longDescription
</pre></p>""" .

ltiv:Group.parentId rdf:type ltiv:Variable ;
  rdfs:comment """An identifier for the parent group within which the target group is nested.
<p>In the LIS Database, this value corresponds to 
<pre>groupRecord/group/relationship[relation=\"Parent\"]/sourcedId
</pre></p>""" .

ltiv:Membership.sourcedId rdf:type ltiv:Variable ;
  rdfs:comment """The LIS identifier for the Membership.
<p>In the LIS Database, this value corresponds to 
<pre>membershipRecord/sourcedId
</pre></p>""" .

ltiv:Membership.collectionSourcedId rdf:type ltiv:Variable ;
  rdfs:comment """The LIS identifier for the organizational unit (Course Section, Group, etc.) to which the Membership pertains.
<p>In the LIS Database, this value corresponds to 
<pre>membershipRecord/membership/collectionSourcedId
</pre></p>""" .

ltiv:Membership.personSourcedId rdf:type ltiv:Variable ;
  rdfs:comment """The LIS identifier for the Person associated with the Membership.
<p>In the LIS Database, this value corresponds to 
<pre>membershipRecord/membership/member/personSourcedId
</pre></p>""" .

ltiv:Membership.status rdf:type ltiv:Variable ;
  rdfs:comment """Indicates if the membership is active or inactive.  In accordance with the LIS specification, the value should be either <code>Active</code> or <code>Inactive</code>.  If the Person has more than one role within the organizational unit, then this value is a comma separated list, where the values are ordered in correspondence with the roles named by the Membership.role variable.
<p>In the LIS Database, this value corresponds to 
<pre>membershipRecord/membership/member/role/status
</pre></p>""" .

ltiv:Membership.createdTimestamp rdf:type ltiv:Variable ;
  rdfs:comment """The date and time when the membership role was created.  If the Person has more than one role within the organizational unit, then this value is a comma separated list corresponding to the roles listed by the Membership.role variable.
<p>In the LIS Database, this value corresponds to 
<pre>membershipRecord/membership/member/role/dateTime
</pre></p>""" .

ltiv:Membership.dataSource rdf:type ltiv:Variable ;
  rdfs:comment """An identifier for the original source system of the Membership record.
<p>In the LIS Database, this value corresponds to 
<pre>membershipRecord/membership/member/role/dataSource
</pre></p>""" .

ltiv:Membership.role rdf:type ltiv:Variable ;
  rdfs:comment """A comma separated list of roles that the Person has within the organizational unit.
<p>In the LIS Database, this value corresponds to 
<pre>membershipRecord/membership/member/role/roleType
</pre></p>""" .

ltiv:LineItemZZZ.sourcedId rdf:type ltiv:Variable ;
  rdfs:comment """The LIS identifier for the LineItem
<p>In the LIS Database, this value corresponds to 
<pre>lineItemRecord/sourcedId
</pre></p>""" .

ltiv:LineItemZZZ.type rdf:type ltiv:Variable ;
  rdfs:comment """A URI that uniquely identifies the LineItem type.  This convention differs from the LIS convention of using a structured object to describe LineItem types.   The URI <em>should</em> resolve to a JSON-LD resource that describes the LineItem type.  As a best practice the URI should start with a base URL that identifies the LineItemType vocabulary and end with a relative URL for a type within that vocabulary.
<p>In the LIS Database, the LineItem type is given by 
<pre>lineItemRecord/lineItem/lineItemType
</pre></p>""" .

ltiv:LineItemZZZ.type.displayName rdf:type ltiv:Variable ;
  rdfs:comment """The display name for the LineItemType.
<p>In the LIS Database, this value corresponds to 
<pre>lineItemTypeRecord/lineItemType/displayName
</pre></p>""" .

ltiv:LineItemZZZ.resultValue.max rdf:type ltiv:Variable ;
  rdfs:comment """The maximum numeric score that a learner may earn on the assignment associated with this LineItem.
<p>In the LIS Database, this value corresponds to 
<pre>resultValueRecord/resultValue/valueRange/max
</pre></p>
<p>where
<pre>resultValueRecord.sourcedId = lineItemRecord/lineItem/resultValueSourcedId
</p>""" .

ltiv:LineItemZZZ.dataSource rdf:type ltiv:Variable ;
  rdfs:comment """An identifier for the original source system of the LineItem record.
<p>In the LIS Database, this value corresponds to 
<pre>lineItemRecord/lineItem/dataSource
</pre></p>""" .

ltiv:Result.sourcedId rdf:type ltiv:Variable ;
  rdfs:comment """The LIS identifier for the Result resource.
<p>In the LIS Database, this value corresponds to 
<pre>
</pre></p>""" .

ltiv:Result.createdTimestamp rdf:type ltiv:Variable ;
  rdfs:comment """The date and time when the Result was created.
<p>In the LIS Database, this value corresponds to 
<pre>
</pre></p>""" .

ltiv:Result.status rdf:type ltiv:Variable ;
  rdfs:comment """A URI for the status of the Result.    As a best practice, the URI <em>should</em> resolve to a JSON-LD description of the status value or a term in a VDEX file.   The vocabulary for Result status values is extensible.  The set of standard values includes:
<UL>
  <LI> http://www.imsglobal.org/lis/omsv1p0/statusofresultvocabularyv1p0#Unmoderated
  <LI> http://www.imsglobal.org/lis/omsv1p0/statusofresultvocabularyv1p0#Tobemoderated
  <LI> http://www.imsglobal.org/lis/omsv1p0/statusofresultvocabularyv1p0#Pending
  <LI> http://www.imsglobal.org/lis/omsv1p0/statusofresultvocabularyv1p0#Completed
</UL>
""" .

ltiv:Result.resultScore rdf:type ltiv:Variable ;
  rdfs:comment """The score that the learner earned on the assignment or activity to which this Result pertains.
<p>In the LIS Database, this value corresponds to 
<pre>resultRecord/result/resultScore/textString
</pre></p>""" .

ltiv:Result.dataSource rdf:type ltiv:Variable ;
  rdfs:comment """An identifier for the original source system of the Result record.
<p>In the LIS Database, this value corresponds to 
<pre>resultRecord/result/dataSource
</pre></p>""" .

ltiv:Result.url rdf:type ltiv:Variable ;
  rdfs:comment "The URL of the Result resource.  Client applications may issue an HTTP request to read, update or delete the resource at this URL." .

ltiv:User.username rdf:type ltiv:Variable ;
  rdfs:comment "The username that identifies the user within the Tool Consumer system." .

ltiv:User.org rdf:type ltiv:Variable ;
  rdfs:comment "A URI describing the user's organisational properties; for example, an ldap:// URI such as <pre>ldap://host.com:6666/uid=user,ou=people,dc=example,dc=com</pre>.  If more than one format of organisational URI is specified, each should be separated with a space." .

ltiv:ResourceLink.description rdf:type ltiv:Variable ;
  rdfs:comment "A plain text description of the link\u2019s destination, suitable for display alongside the link." .

ltiv:ResourceLink.title rdf:type ltiv:Variable ;
  rdfs:comment "A plain text title for the resource." .

ltiv:Context.org rdf:type ltiv:Variable ;
  rdfs:comment "A URI describing the organisational properties of the context from which a launch request originates (typically a CourseSection); for example, an ldap:// URI such as <pre>ldap://host.com:6666/cid=abc123,ou=dept,dc=plainjoe,dc=org</pre>. If more than one format of organisational URI is specified, each should be separated with a space." .

ltiv:ToolProxy.custom.url rdf:type ltiv:Variable ;
  rdfs:comment "The endpoint URL for accessing system-wide tool settings." .

ltiv:ToolProxyBinding.custom.url rdf:type ltiv:Variable ;
  rdfs:comment "The endpoint URL for accessing context-level tool settings." .

ltiv:LtiLink.custom.url rdf:type ltiv:Variable ;
  rdfs:comment "The endpoint URL for accessing link-level tool settings." .

ltiv:Result.comment rdf:type ltiv:Variable ;
  rdfs:comment "A comment associated with the outcome which may be made visible to the student." .

ltiv:User.scope.mentor rdf:type ltiv:Variable ;
  rdfs:comment "A comma-separated list of user ID values which the current user can access as a mentor.    Corresponds to the role_scope_mentor launch parameter." .

ltiv:Context.id rdf:type ltiv:Variable ;
  rdfs:comment "Corresponds to the context_id launch parameter.  This is the local identifier for the context within the Tool Consumer system." .

ltiv:Context.type rdf:type ltiv:Variable ;
  rdfs:comment "A comma-separated list of URN values that identify the type of context.  Corresponds to the context_type launch parameter." .

ltiv:Context.title rdf:type ltiv:Variable ;
  rdfs:comment "The title for the context.  Corresponds to the context_title launch parameter." .

ltiv:Context.label rdf:type ltiv:Variable ;
  rdfs:comment "A short label for the context.  Corresponds to the context_label launch parameter." .

ltiv:ResourceLink.id rdf:type ltiv:Variable ;
  rdfs:comment "This is the local identifier for the resource link within the Tool Consumer system from which the launch occurred.  Corresponds to the resource_link_id launch parameter." .
@prefix rdf: <http://www.w3.org/1999/02/22-rdf-syntax-ns#> .
@prefix rdfs: <http://www.w3.org/2000/01/rdf-schema#> .
@prefix bind: <http://purl.org/semantictools/v1/vocab/bind#> .
@prefix ltiv: <http://ld.kinexis.com/vocab/lti/v2/variable#> .

ltiv:Variable rdf:type bind:Enum .
@prefix ltic: <http://ld.kinexis.com/vocab/lti/v2/capability#> .
@prefix lti: <http://ld.kinexis.com/vocab/lti/v2/lti#> .
@prefix owl: <http://www.w3.org/2002/07/owl#> .
@prefix rdf: <http://www.w3.org/1999/02/22-rdf-syntax-ns#> .
@prefix rdfs: <http://www.w3.org/2000/01/rdf-schema#> .
@prefix xsd: <http://www.w3.org/2001/XMLSchema#> .
@prefix bind: <http://purl.org/semantictools/v1/vocab/bind#> .

<http://ld.kinexis.com/vocab/lti/v2/capability#> a owl:Ontology  ;
  rdfs:label "LTI Capabilities" ;
  a bind:TargetNamespace ;
  bind:suggestedPrefix "ltic" .

ltic:OutcomesCapability rdf:type owl:Class ;
  rdfs:subClassOf lti:Capability ; 
  rdfs:comment "Capabilities to support services relating to Outcomes." .

ltic:Result.autocreate rdf:type ltic:OutcomesCapability ;
  rdfs:comment "A lin-item in the tool consumer gradebook can be automatically created for any resource links which use the Basic Outcomes or Result services." .
@prefix rdf: <http://www.w3.org/1999/02/22-rdf-syntax-ns#> .
@prefix rdfs: <http://www.w3.org/2000/01/rdf-schema#> .
@prefix bind: <http://purl.org/semantictools/v1/vocab/bind#> .
@prefix ltic: <http://ld.kinexis.com/vocab/lti/v2/capability#> .

@prefix rdfs: <http://www.w3.org/2000/01/rdf-schema#> .
@prefix owl: <http://www.w3.org/2002/07/owl#> .
@prefix rdf: <http://www.w3.org/1999/02/22-rdf-syntax-ns#> .
@prefix xsd: <http://www.w3.org/2001/XMLSchema#> .
@prefix bind: <http://purl.org/semantictools/v1/vocab/bind#> .

<http://www.w3.org/2000/01/rdf-schema#> a owl:Ontology  ;
  rdfs:label "RDF Schema" ;
  a bind:TargetNamespace ;
  bind:suggestedPrefix "rdfs" .

rdfs:Resource rdf:type owl:Class .
@prefix rdf: <http://www.w3.org/1999/02/22-rdf-syntax-ns#> .
@prefix rdfs: <http://www.w3.org/2000/01/rdf-schema#> .
@prefix bind: <http://purl.org/semantictools/v1/vocab/bind#> .
@prefix rdfs: <http://www.w3.org/2000/01/rdf-schema#> .

rdfs:Resource rdf:type bind:Addressable .
@prefix exp: <http://ld.kinexis.com/vocab/caliper/v1/core#> .
@prefix xsd: <http://www.w3.org/2001/XMLSchema#> .
@prefix owl: <http://www.w3.org/2002/07/owl#> .
@prefix rdf: <http://www.w3.org/1999/02/22-rdf-syntax-ns#> .
@prefix rdfs: <http://www.w3.org/2000/01/rdf-schema#> .
@prefix bind: <http://purl.org/semantictools/v1/vocab/bind#> .

<http://ld.kinexis.com/vocab/caliper/v1/core#> a owl:Ontology  ;
  rdfs:label "Caliper Core" ;
  a bind:TargetNamespace ;
  bind:suggestedPrefix "exp" .

exp:Activity rdf:type owl:Class;
  rdfs:subClassOf 
  [ a owl:Restriction ;
    owl:onProperty      exp:activityId;
    owl:minCardinality  1;
    rdfs:comment "The unique ID for the activity as used by the tool provider."
  ] ; 
  rdfs:comment "A resource that a person may experience such as a video or an assessment.  This entity represents the resource itself, not the person's engagement with the resource." .

exp:activityId rdf:type owl:FunctionalProperty ;
  rdfs:domain exp:Activity ;
  rdfs:range xsd:normalizedString ;
  rdfs:comment "The unique ID for the activity as used by the tool provider." .
@prefix rdf: <http://www.w3.org/1999/02/22-rdf-syntax-ns#> .
@prefix rdfs: <http://www.w3.org/2000/01/rdf-schema#> .
@prefix bind: <http://purl.org/semantictools/v1/vocab/bind#> .
@prefix exp: <http://ld.kinexis.com/vocab/caliper/v1/core#> .

exp:Activity rdf:type bind:Addressable .
@prefix ldp: <http://www.w3.org/ns/ldp#> .
@prefix rdf: <http://www.w3.org/1999/02/22-rdf-syntax-ns#> .
@prefix rdfs: <http://www.w3.org/2000/01/rdf-schema#> .
@prefix owl: <http://www.w3.org/2002/07/owl#> .
@prefix xsd: <http://www.w3.org/2001/XMLSchema#> .
@prefix bind: <http://purl.org/semantictools/v1/vocab/bind#> .

<http://www.w3.org/ns/ldp#> a owl:Ontology  ;
  rdfs:label "W3C Linked Data Platform" ;
  a bind:TargetNamespace ;
  bind:suggestedPrefix "ldp" .

ldp:Container rdf:type owl:Class;
  rdfs:subClassOf 
  [ a owl:Restriction ;
    owl:onProperty      ldp:membershipPredicate;
    owl:minCardinality  1;
    rdfs:comment "Indicates which predicate of the container's subject should be used to determine membership in the container."
  ] ,
  [ a owl:Restriction ;
    owl:onProperty      ldp:membershipSubject;
    owl:minCardinality  1;
    rdfs:comment "Indicates which resource is the subject for the members of the container."
  ] ; 
  rdfs:comment "A container that holds a collection of resources.  New resources are added to the container by submitting an HTTP POST request to the container endpoint. " .

ldp:Page rdf:type owl:Class;
  rdfs:subClassOf 
  [ a owl:Restriction ;
    owl:onProperty      ldp:pageOf;
    owl:minCardinality  1;
    rdfs:comment "Associates a page with its container."
  ] ,
  [ a owl:Restriction ;
    owl:onProperty      ldp:nextPage;
    owl:minCardinality  1;
    rdfs:comment "A URL to the next page of results."
  ] ; 
  rdfs:comment "A resource that represents a limited set of members of a LDP Container." .

ldp:membershipPredicate rdf:type owl:FunctionalProperty ;
  rdfs:domain ldp:Container ;
  rdfs:range rdf:Property ;
  rdfs:comment "Indicates which predicate of the container's subject should be used to determine membership in the container." .

ldp:membershipSubject rdf:type owl:FunctionalProperty ;
  rdfs:domain ldp:Container ;
  rdfs:range rdfs:Resource ;
  rdfs:comment "Indicates which resource is the subject for the members of the container." .

ldp:pageOf rdf:type owl:FunctionalProperty ;
  rdfs:domain ldp:Page ;
  rdfs:range ldp:Container ;
  rdfs:comment "Associates a page with its container." .

ldp:nextPage rdf:type owl:FunctionalProperty ;
  rdfs:domain ldp:Page ;
  rdfs:range ldp:Page ;
  rdfs:comment "A URL to the next page of results." .
@prefix rdf: <http://www.w3.org/1999/02/22-rdf-syntax-ns#> .
@prefix rdfs: <http://www.w3.org/2000/01/rdf-schema#> .
@prefix bind: <http://purl.org/semantictools/v1/vocab/bind#> .
@prefix ldp: <http://www.w3.org/ns/ldp#> .

ldp:Container rdf:type bind:Addressable .
ldp:Container rdfs:subClassOf
  [ rdf:type bind:AssociationQualifier ;
    bind:onProperty ldp:membershipPredicate ;
    bind:associationType bind:Aggregation
  ], 
  [ rdf:type bind:AssociationQualifier ;
    bind:onProperty ldp:membershipSubject ;
    bind:associationType bind:Aggregation
  ] .
ldp:Page rdf:type bind:Addressable .
ldp:Page rdfs:subClassOf
  [ rdf:type bind:AssociationQualifier ;
    bind:onProperty ldp:pageOf ;
    bind:inverseAssociationType bind:Composition
  ], 
  [ rdf:type bind:AssociationQualifier ;
    bind:onProperty ldp:nextPage ;
    bind:associationType bind:Aggregation
  ] .
@prefix ci: <http://ld.kinexis.com/vocab/lti/v1/ci#> .
@prefix xsd: <http://www.w3.org/2001/XMLSchema#> .
@prefix lti: <http://ld.kinexis.com/vocab/lti/v2/lti#> .
@prefix liso: <http://ld.kinexis.com/vocab/lis/v2/outcomes#> .
@prefix owl: <http://www.w3.org/2002/07/owl#> .
@prefix rdf: <http://www.w3.org/1999/02/22-rdf-syntax-ns#> .
@prefix rdfs: <http://www.w3.org/2000/01/rdf-schema#> .
@prefix bind: <http://purl.org/semantictools/v1/vocab/bind#> .

<http://ld.kinexis.com/vocab/lti/v1/ci#> a owl:Ontology  ;
  rdfs:label "Content-Item Message" ;
  a bind:TargetNamespace ;
  bind:suggestedPrefix "ci" .

ci:ContentItemPlacement rdf:type owl:Class;
  rdfs:subClassOf 
  [ a owl:Restriction ;
    owl:onProperty      ci:displayWidth;
    rdfs:comment "The width in pixels of the display area."
  ] ,
  [ a owl:Restriction ;
    owl:onProperty      ci:displayHeight;
    rdfs:comment "The height in pixels of the display area."
  ] ,
  [ a owl:Restriction ;
    owl:onProperty      ci:windowTarget;
    rdfs:comment "The value for the <code>target</code> attribute of any anchor tag which is used to make the content-item available to users."
  ] ,
  [ a owl:Restriction ;
    owl:onProperty      ci:presentationDocumentTarget;
    rdfs:comment "The intended destination where the content-item is displayed to users.  The value is taken from a list of permitted targets."
  ] ; 
  rdfs:comment "A class identifying how a content item should be displayed." .

ci:ContentItem rdf:type owl:Class;
  rdfs:subClassOf 
  [ a owl:Restriction ;
    owl:onProperty      ci:mediaType;
    owl:minCardinality  1;
    rdfs:comment "The MIME type of the content-item."
  ] ,
  [ a owl:Restriction ;
    owl:onProperty      ci:title;
    rdfs:comment "A plain text title of the content-item."
  ] ,
  [ a owl:Restriction ;
    owl:onProperty      ci:text;
    rdfs:comment "A plain text description of the content-item."
  ] ,
  [ a owl:Restriction ;
    owl:onProperty      ci:url;
    rdfs:comment "The URL at which the content item is located."
  ] ,
  [ a owl:Restriction ;
    owl:onProperty      ci:placementAdvice;
    rdfs:comment "Suggestion for how the item should be placed for user display."
  ] ,
  [ a owl:Restriction ;
    owl:onProperty      ci:thumbnail;
    rdfs:comment "An image which may be used as a thumbnail for the content-item."
  ] ,
  [ a owl:Restriction ;
    owl:onProperty      ci:icon;
    rdfs:comment "An image which may be used as an icon for the content-item."
  ] ; 
  rdfs:comment "A class representing a content item." .

ci:Image rdf:type owl:Class;
  rdfs:subClassOf 
  [ a owl:Restriction ;
    owl:onProperty      ci:width;
    rdfs:comment "The width in pixels of the image."
  ] ,
  [ a owl:Restriction ;
    owl:onProperty      ci:height;
    rdfs:comment "The height in pixels of the image."
  ] ; 
  rdfs:comment "Dimensions for an item representing an image." .

ci:FileItem rdf:type owl:Class ;
  rdfs:subClassOf ci:ContentItem ,
  [ a owl:Restriction ;
    owl:onProperty      ci:copyAdvice;
    rdfs:comment "Whether a copy of the item should be made available locally for continued access."
  ] ,
  [ a owl:Restriction ;
    owl:onProperty      ci:expiresAt;
    rdfs:comment "The time until which access to this item is available."
  ] ; 
  rdfs:comment "A content-item representing a file which needs to be copied locally for persistent access." .

ci:LtiLinkItem rdf:type owl:Class ;
  rdfs:subClassOf ci:ContentItem ,
  [ a owl:Restriction ;
    owl:onProperty      ci:custom;
    rdfs:comment "Custom parameters (name and value pairs) which are associated with the LTI link."
  ] ; 
  rdfs:comment "An LTI resource link." .

ci:AssignmentLinkItem rdf:type owl:Class ;
  rdfs:subClassOf ci:LtiLinkItem ,
  [ a owl:Restriction ;
    owl:onProperty      ci:assignmentLineItem;
    owl:minCardinality  1;
    rdfs:comment "LineItem for an LTI link which is assessable."
  ] ; 
  rdfs:comment "An LTI resource link which has an associated line-item." .

ci:displayWidth rdf:type owl:FunctionalProperty ;
  rdfs:domain ci:ContentItemPlacement ;
  rdfs:range xsd:integer ;
  rdfs:comment "The width in pixels of the display area." .

ci:displayHeight rdf:type owl:FunctionalProperty ;
  rdfs:domain ci:ContentItemPlacement ;
  rdfs:range xsd:integer ;
  rdfs:comment "The height in pixels of the display area." .

ci:windowTarget rdf:type owl:FunctionalProperty ;
  rdfs:domain ci:ContentItemPlacement ;
  rdfs:range xsd:normalizedString ;
  rdfs:comment "The value for the <code>target</code> attribute of any anchor tag which is used to make the content-item available to users." .

ci:presentationDocumentTarget rdf:type owl:FunctionalProperty ;
  rdfs:domain ci:ContentItemPlacement ;
  rdfs:range lti:DocumentTarget ;
  rdfs:comment "The intended destination where the content-item is displayed to users.  The value is taken from a list of permitted targets." .

ci:mediaType rdf:type owl:FunctionalProperty ;
  rdfs:domain ci:ContentItem ;
  rdfs:range xsd:normalizedString ;
  rdfs:comment "The MIME type of the content-item." .

ci:title rdf:type owl:FunctionalProperty ;
  rdfs:domain ci:ContentItem ;
  rdfs:range xsd:normalizedString ;
  rdfs:comment "A plain text title of the content-item." .

ci:text rdf:type owl:FunctionalProperty ;
  rdfs:domain ci:ContentItem ;
  rdfs:range xsd:string ;
  rdfs:comment "A plain text description of the content-item." .

ci:url rdf:type owl:FunctionalProperty ;
  rdfs:domain ci:ContentItem ;
  rdfs:range xsd:anyURI ;
  rdfs:comment "The URL at which the content item is located." .

ci:placementAdvice rdf:type owl:FunctionalProperty ;
  rdfs:domain ci:ContentItem ;
  rdfs:range ci:ContentItemPlacement ;
  rdfs:comment "Suggestion for how the item should be placed for user display." .

ci:thumbnail rdf:type owl:FunctionalProperty ;
  rdfs:domain ci:ContentItem ;
  rdfs:range ci:Image ;
  rdfs:comment "An image which may be used as a thumbnail for the content-item." .

ci:icon rdf:type owl:FunctionalProperty ;
  rdfs:domain ci:ContentItem ;
  rdfs:range ci:Image ;
  rdfs:comment "An image which may be used as an icon for the content-item." .

ci:width rdf:type owl:FunctionalProperty ;
  rdfs:domain ci:Image ;
  rdfs:range xsd:integer ;
  rdfs:comment "The width in pixels of the image." .

ci:height rdf:type owl:FunctionalProperty ;
  rdfs:domain ci:Image ;
  rdfs:range xsd:integer ;
  rdfs:comment "The height in pixels of the image." .

ci:copyAdvice rdf:type owl:FunctionalProperty ;
  rdfs:domain ci:FileItem ;
  rdfs:range xsd:boolean ;
  rdfs:comment "Whether a copy of the item should be made available locally for continued access." .

ci:expiresAt rdf:type owl:FunctionalProperty ;
  rdfs:domain ci:FileItem ;
  rdfs:range xsd:dateTime ;
  rdfs:comment "The time until which access to this item is available." .

ci:custom rdf:type owl:FunctionalProperty ;
  rdfs:domain ci:LtiLinkItem ;
  rdfs:range lti:PropertyMap ;
  rdfs:comment "Custom parameters (name and value pairs) which are associated with the LTI link." .

ci:assignmentLineItem rdf:type owl:FunctionalProperty ;
  rdfs:domain ci:AssignmentLinkItem ;
  rdfs:range liso:LineItem ;
  rdfs:comment "LineItem for an LTI link which is assessable." .
@prefix rdf: <http://www.w3.org/1999/02/22-rdf-syntax-ns#> .
@prefix rdfs: <http://www.w3.org/2000/01/rdf-schema#> .
@prefix bind: <http://purl.org/semantictools/v1/vocab/bind#> .
@prefix ci: <http://ld.kinexis.com/vocab/lti/v1/ci#> .

ci:ContentItemPlacement rdfs:subClassOf
  [ rdf:type bind:AssociationQualifier ;
    bind:onProperty ci:presentationDocumentTarget
  ] .
ci:ContentItem rdf:type bind:Addressable .
ci:ContentItem rdfs:subClassOf
  [ rdf:type bind:AssociationQualifier ;
    bind:onProperty ci:placementAdvice
  ], 
  [ rdf:type bind:AssociationQualifier ;
    bind:onProperty ci:thumbnail
  ], 
  [ rdf:type bind:AssociationQualifier ;
    bind:onProperty ci:icon
  ] .
ci:Image rdf:type bind:Addressable .
ci:FileItem rdf:type bind:Addressable .
ci:LtiLinkItem rdf:type bind:Addressable .
ci:LtiLinkItem rdfs:subClassOf
  [ rdf:type bind:AssociationQualifier ;
    bind:onProperty ci:custom ;
    bind:associationType bind:Composition
  ] .
ci:AssignmentLinkItem rdf:type bind:Addressable .
ci:AssignmentLinkItem rdfs:subClassOf
  [ rdf:type bind:AssociationQualifier ;
    bind:onProperty ci:assignmentLineItem
  ] .
@prefix foaf: <http://xmlns.com/foaf/0.1#> .
@prefix org: <http://www.w3.org/ns/org#> .
@prefix owl: <http://www.w3.org/2002/07/owl#> .
@prefix rdf: <http://www.w3.org/1999/02/22-rdf-syntax-ns#> .
@prefix rdfs: <http://www.w3.org/2000/01/rdf-schema#> .
@prefix xsd: <http://www.w3.org/2001/XMLSchema#> .
@prefix bind: <http://purl.org/semantictools/v1/vocab/bind#> .

<http://xmlns.com/foaf/0.1#> a owl:Ontology  ;
  rdfs:label "FOAF" ;
  a bind:TargetNamespace ;
  bind:suggestedPrefix "foaf" .

foaf:Agent rdf:type owl:Class;
  rdfs:subClassOf 
  [ a owl:Restriction ;
    owl:onProperty      org:hasMembership;
    rdfs:comment "Indicates a membership relationship that the Agent plays."
  ] ; 
  rdfs:comment "An agent (eg. person, group, software or physical artifact)." .
@prefix rdf: <http://www.w3.org/1999/02/22-rdf-syntax-ns#> .
@prefix rdfs: <http://www.w3.org/2000/01/rdf-schema#> .
@prefix bind: <http://purl.org/semantictools/v1/vocab/bind#> .
@prefix foaf: <http://xmlns.com/foaf/0.1#> .

foaf:Agent rdf:type bind:Addressable .
@prefix lisp: <http://ld.kinexis.com/vocab/lis/v2/pm#> .
@prefix xsd: <http://www.w3.org/2001/XMLSchema#> .
@prefix schema: <http://schema.org/> .
@prefix owl: <http://www.w3.org/2002/07/owl#> .
@prefix rdf: <http://www.w3.org/1999/02/22-rdf-syntax-ns#> .
@prefix rdfs: <http://www.w3.org/2000/01/rdf-schema#> .
@prefix bind: <http://purl.org/semantictools/v1/vocab/bind#> .

<http://ld.kinexis.com/vocab/lis/v2/pm#> a owl:Ontology  ;
  rdfs:label "LIS Person Management" ;
  a bind:TargetNamespace ;
  bind:suggestedPrefix "lisp" .

lisp:LISPerson rdf:type owl:Class ;
  rdfs:subClassOf schema:Person ,
  [ a owl:Restriction ;
    owl:onProperty      lisp:userId;
    owl:minCardinality  1;
    rdfs:comment "A unique identifier for the person."
  ] ,
  [ a owl:Restriction ;
    owl:onProperty      lisp:sourcedId;
    rdfs:comment "A unique identifier for the person as provisioned by an external system such as an SIS."
  ] ,
  [ a owl:Restriction ;
    owl:onProperty      lisp:email;
    rdfs:comment "The primary email address for the person."
  ] ,
  [ a owl:Restriction ;
    owl:onProperty      lisp:resultSourcedId;
    rdfs:comment "The person's LIS Result Identifier (if any) associated with a launch from the organization.  This will normally only have a value if the organization represents a resource link, though could also reflect a course-level launch."
  ] ; 
  rdfs:comment "A container for all the information about a single person." .

lisp:userId rdf:type owl:FunctionalProperty ;
  rdfs:domain lisp:LISPerson ;
  rdfs:range xsd:normalizedString ;
  rdfs:comment "A unique identifier for the person." .

lisp:sourcedId rdf:type owl:FunctionalProperty ;
  rdfs:domain lisp:LISPerson ;
  rdfs:range xsd:normalizedString ;
  rdfs:comment "A unique identifier for the person as provisioned by an external system such as an SIS." .

lisp:email rdf:type owl:FunctionalProperty ;
  rdfs:domain lisp:LISPerson ;
  rdfs:range xsd:string ;
  rdfs:comment "The primary email address for the person." .

lisp:resultSourcedId rdf:type owl:FunctionalProperty ;
  rdfs:domain lisp:LISPerson ;
  rdfs:range xsd:string ;
  rdfs:comment "The person's LIS Result Identifier (if any) associated with a launch from the organization.  This will normally only have a value if the organization represents a resource link, though could also reflect a course-level launch." .
@prefix rdf: <http://www.w3.org/1999/02/22-rdf-syntax-ns#> .
@prefix rdfs: <http://www.w3.org/2000/01/rdf-schema#> .
@prefix bind: <http://purl.org/semantictools/v1/vocab/bind#> .
@prefix lisp: <http://ld.kinexis.com/vocab/lis/v2/pm#> .

lisp:LISPerson rdf:type bind:Addressable .
@prefix liso: <http://ld.kinexis.com/vocab/lis/v2/outcomes#> .
@prefix xsd: <http://www.w3.org/2001/XMLSchema#> .
@prefix rdf: <http://www.w3.org/1999/02/22-rdf-syntax-ns#> .
@prefix lti: <http://ld.kinexis.com/vocab/lti/v2/lti#> .
@prefix exp: <http://ld.kinexis.com/vocab/caliper/v1/core#> .
@prefix rdfs: <http://www.w3.org/2000/01/rdf-schema#> .
@prefix lti-type: <http://ld.kinexis.com/xsd/lti/v2/ltid#> .
@prefix lisp: <http://ld.kinexis.com/vocab/lis/v2/pm#> .
@prefix foaf: <http://xmlns.com/foaf/0.1#> .
@prefix ldp: <http://www.w3.org/ns/ldp#> .
@prefix owl: <http://www.w3.org/2002/07/owl#> .
@prefix bind: <http://purl.org/semantictools/v1/vocab/bind#> .

<http://ld.kinexis.com/vocab/lis/v2/outcomes#> a owl:Ontology  ;
  rdfs:label "LIS Outcomes" ;
  a bind:TargetNamespace ;
  bind:suggestedPrefix "liso" .

liso:LISResult rdf:type owl:Class ;
  rdfs:subClassOf liso:AbstractResult ,
  [ a owl:Restriction ;
    owl:onProperty      liso:normalScore;
    rdfs:comment "The score earned by the learner before adding extra credit or subtracting penalties."
  ] ,
  [ a owl:Restriction ;
    owl:onProperty      liso:extraCreditScore;
    rdfs:comment "The number of exta credit points earned by the learner."
  ] ,
  [ a owl:Restriction ;
    owl:onProperty      liso:penaltyScore;
    rdfs:comment "The number of points deducted from the normal score due to some penalty such as submitting an assignment after the due date."
  ] ,
  [ a owl:Restriction ;
    owl:onProperty      liso:totalScore;
    rdfs:comment """The total score on the assignment given by
<pre>
    totalScore = normalScore + extraCreditScore - penalty
</pre>
This value does not take into account the effects of curving.
"""
  ] ,
  [ a owl:Restriction ;
    owl:onProperty      liso:timestamp;
    rdfs:comment "The time at which the result was generated."
  ] ,
  [ a owl:Restriction ;
    owl:onProperty      liso:resultOf;
    owl:minCardinality  1;
    rdfs:comment "The LineItem within which this Result is contained."
  ] ,
  [ a owl:Restriction ;
    owl:onProperty      liso:resultStatus;
    rdfs:comment "The status of the result for this user and line item."
  ] ,
  [ a owl:Restriction ;
    owl:onProperty      liso:resultScoreConstraints;
    rdfs:comment "Constraints on the scores recorded in this Result."
  ] ; 
  rdfs:comment "A container that holds the result of some scorable activity or assignment." .

liso:LineItem rdf:type owl:Class;
  rdfs:subClassOf 
  [ a owl:Restriction ;
    owl:onProperty      liso:label;
    rdfs:comment "A human-friendly label for this LineItem suitable for display.  For example, this label might be used as the heading of a column in a gradebook."
  ] ,
  [ a owl:Restriction ;
    owl:onProperty      liso:reportingMethod;
    owl:minCardinality  1;
    rdfs:comment "Identifies the property that is reported as the <code>resultScore</code> of the Results within this LineItem."
  ] ,
  [ a owl:Restriction ;
    owl:onProperty      liso:result;
    rdfs:comment "A Result associated with this LineItem."
  ] ,
  [ a owl:Restriction ;
    owl:onProperty      liso:scoreConstraints;
    rdfs:comment "Constraints on the scores recorded in the Results associated with this LineItem."
  ] ,
  [ a owl:Restriction ;
    owl:onProperty      liso:lineItemOf;
    owl:minCardinality  1;
    rdfs:comment "The context to which this LineItem belongs."
  ] ,
  [ a owl:Restriction ;
    owl:onProperty      liso:results;
    owl:minCardinality  1;
    rdfs:comment "The container holding the Results for this LineItem.  "
  ] ,
  [ a owl:Restriction ;
    owl:onProperty      liso:assignedActivity;
    rdfs:comment "The Activity that learners engage with to produce the Results recorded in this LineItem."
  ] ,
  [ a owl:Restriction ;
    owl:onProperty      liso:dataSource;
    rdfs:comment "The resource associated with this line item."
  ] ; 
  rdfs:comment "A class representing a column in a gradebook capable of holding result values for different users for a single activity." .

liso:ScoreConstraints rdf:type owl:Class ; 
  rdfs:comment "The abstract base class for all the various kinds of constraints that might be imposed on the Results associated with a LineItem." .

liso:NumericLimits rdf:type owl:Class ;
  rdfs:subClassOf liso:ScoreConstraints ,
  [ a owl:Restriction ;
    owl:onProperty      liso:normalMaximum;
    rdfs:comment "The maximum number of points that a learner may earn without extra credit."
  ] ,
  [ a owl:Restriction ;
    owl:onProperty      liso:extraCreditMaximum;
    rdfs:comment "The maximum number of extra credit points that a learner may earn."
  ] ,
  [ a owl:Restriction ;
    owl:onProperty      liso:totalMaximum;
    rdfs:comment """The maximum number of points that a learner may earn.  This value is given by
<pre>
    totalMaximum = normalMaximum + extraCreditMaximum
</pre>"""
  ] ; 
  rdfs:comment "Defines the maximum values for numerical scores." .

liso:ResultContainer rdf:type owl:Class ;
  rdfs:subClassOf ldp:Container ,
  [ a owl:Restriction ;
    owl:onProperty      ldp:membershipPredicate;
    owl:hasValue liso:result
  ] ,
  [ a owl:Restriction ;
    owl:onProperty      ldp:membershipSubject;
    owl:allValuesFrom  liso:LineItem
  ] ; 
  rdfs:comment "A container that holds a collection of Result resources." .

liso:LineItemContainer rdf:type owl:Class ;
  rdfs:subClassOf ldp:Container ,
  [ a owl:Restriction ;
    owl:onProperty      ldp:membershipPredicate;
    owl:hasValue lti:lineItem
  ] ,
  [ a owl:Restriction ;
    owl:onProperty      ldp:membershipSubject;
    owl:allValuesFrom  lti:Context
  ] ; 
  rdfs:comment "A container that holds a collection of LineItem resources." .

liso:Result rdf:type owl:Class ;
  rdfs:subClassOf liso:AbstractResult ; 
  rdfs:comment "A basic result resource." .

liso:ResultStatus rdf:type owl:Class ; 
  rdfs:comment "Possible status values for result resources." .

liso:AbstractResult rdf:type owl:Class;
  rdfs:subClassOf 
  [ a owl:Restriction ;
    owl:onProperty      liso:resultScore;
    rdfs:comment "The final score that should be displayed in a gradebook for this Result object."
  ] ,
  [ a owl:Restriction ;
    owl:onProperty      liso:comment;
    rdfs:comment "A comment about this Result suitable for display to the learner. Typically, this is a comment made by the instructor or grader."
  ] ,
  [ a owl:Restriction ;
    owl:onProperty      liso:resultAgent;
    owl:minCardinality  1;
    rdfs:comment "The person whose score is recorded in this Result."
  ] ,
  [ a owl:Restriction ;
    owl:onProperty      liso:gradedBy;
    rdfs:comment "The agent who generated the result."
  ] ; 
  rdfs:comment "An abstract class representing common elements for the different classes related to the various Outcomes services." .

liso:normalScore rdf:type owl:FunctionalProperty ;
  rdfs:domain liso:LISResult ;
  rdfs:range xsd:decimal ;
  rdfs:comment "The score earned by the learner before adding extra credit or subtracting penalties." .

liso:extraCreditScore rdf:type owl:FunctionalProperty ;
  rdfs:domain liso:LISResult ;
  rdfs:range xsd:decimal ;
  rdfs:comment "The number of exta credit points earned by the learner." .

liso:penaltyScore rdf:type owl:FunctionalProperty ;
  rdfs:domain liso:LISResult ;
  rdfs:range xsd:decimal ;
  rdfs:comment "The number of points deducted from the normal score due to some penalty such as submitting an assignment after the due date." .

liso:totalScore rdf:type owl:FunctionalProperty ;
  rdfs:domain liso:LISResult ;
  rdfs:range xsd:decimal ;
  rdfs:comment """The total score on the assignment given by
<pre>
    totalScore = normalScore + extraCreditScore - penalty
</pre>
This value does not take into account the effects of curving.
""" .

liso:timestamp rdf:type owl:FunctionalProperty ;
  rdfs:domain liso:LISResult ;
  rdfs:range xsd:dateTime ;
  rdfs:comment "The time at which the result was generated." .

liso:resultOf rdf:type owl:FunctionalProperty ;
  rdfs:domain liso:LISResult ;
  rdfs:range liso:LineItem ;
  owl:inverseOf liso:result ;
  rdfs:comment "The LineItem within which this Result is contained." .

liso:resultStatus rdf:type owl:FunctionalProperty ;
  rdfs:domain liso:LISResult ;
  rdfs:range liso:ResultStatus ;
  rdfs:comment "The status of the result for this user and line item." .

liso:resultScoreConstraints rdf:type owl:FunctionalProperty ;
  rdfs:domain liso:LISResult ;
  rdfs:range liso:ScoreConstraints ;
  rdfs:comment "Constraints on the scores recorded in this Result." .

liso:label rdf:type owl:FunctionalProperty ;
  rdfs:domain liso:LineItem ;
  rdfs:range xsd:normalizedString ;
  rdfs:comment "A human-friendly label for this LineItem suitable for display.  For example, this label might be used as the heading of a column in a gradebook." .

liso:reportingMethod rdf:type owl:FunctionalProperty ;
  rdfs:domain liso:LineItem ;
  rdfs:range rdf:Property ;
  rdfs:comment "Identifies the property that is reported as the <code>resultScore</code> of the Results within this LineItem." .

liso:result rdf:type rdf:Property ;
  rdfs:domain liso:LineItem ;
  rdfs:range liso:LISResult ;
  owl:inverseOf liso:resultOf ;
  rdfs:comment "A Result associated with this LineItem." .

liso:scoreConstraints rdf:type owl:FunctionalProperty ;
  rdfs:domain liso:LineItem ;
  rdfs:range liso:ScoreConstraints ;
  rdfs:comment "Constraints on the scores recorded in the Results associated with this LineItem." .

liso:lineItemOf rdf:type owl:FunctionalProperty ;
  rdfs:domain liso:LineItem ;
  rdfs:range lti:Context ;
  owl:inverseOf lti:lineItem ;
  rdfs:comment "The context to which this LineItem belongs." .

liso:results rdf:type owl:FunctionalProperty ;
  rdfs:domain liso:LineItem ;
  rdfs:range liso:ResultContainer ;
  rdfs:comment "The container holding the Results for this LineItem.  " .

liso:assignedActivity rdf:type owl:FunctionalProperty ;
  rdfs:domain liso:LineItem ;
  rdfs:range exp:Activity ;
  rdfs:comment "The Activity that learners engage with to produce the Results recorded in this LineItem." .

liso:dataSource rdf:type owl:FunctionalProperty ;
  rdfs:domain liso:LineItem ;
  rdfs:range rdfs:Resource ;
  rdfs:comment "The resource associated with this line item." .

liso:normalMaximum rdf:type owl:FunctionalProperty ;
  rdfs:domain liso:NumericLimits ;
  rdfs:range xsd:float ;
  rdfs:comment "The maximum number of points that a learner may earn without extra credit." .

liso:extraCreditMaximum rdf:type owl:FunctionalProperty ;
  rdfs:domain liso:NumericLimits ;
  rdfs:range xsd:float ;
  rdfs:comment "The maximum number of extra credit points that a learner may earn." .

liso:totalMaximum rdf:type owl:FunctionalProperty ;
  rdfs:domain liso:NumericLimits ;
  rdfs:range xsd:float ;
  rdfs:comment """The maximum number of points that a learner may earn.  This value is given by
<pre>
    totalMaximum = normalMaximum + extraCreditMaximum
</pre>""" .

liso:resultScore rdf:type owl:FunctionalProperty ;
  rdfs:domain liso:AbstractResult ;
  rdfs:range rdfs:Literal ;
  rdfs:comment "The final score that should be displayed in a gradebook for this Result object." .

liso:comment rdf:type owl:FunctionalProperty ;
  rdfs:domain liso:AbstractResult ;
  rdfs:range lti-type:DataValue.Type ;
  rdfs:comment "A comment about this Result suitable for display to the learner. Typically, this is a comment made by the instructor or grader." .

liso:resultAgent rdf:type owl:FunctionalProperty ;
  rdfs:domain liso:AbstractResult ;
  rdfs:range lisp:LISPerson ;
  rdfs:comment "The person whose score is recorded in this Result." .

liso:gradedBy rdf:type owl:FunctionalProperty ;
  rdfs:domain liso:AbstractResult ;
  rdfs:range foaf:Agent ;
  rdfs:comment "The agent who generated the result." .

liso:Final rdf:type liso:ResultStatus .

liso:Initialized rdf:type liso:ResultStatus .

liso:Started rdf:type liso:ResultStatus .

liso:Completed rdf:type liso:ResultStatus .
@prefix rdf: <http://www.w3.org/1999/02/22-rdf-syntax-ns#> .
@prefix rdfs: <http://www.w3.org/2000/01/rdf-schema#> .
@prefix bind: <http://purl.org/semantictools/v1/vocab/bind#> .
@prefix liso: <http://ld.kinexis.com/vocab/lis/v2/outcomes#> .

liso:LISResult rdf:type bind:Addressable .
liso:LISResult rdfs:subClassOf
  [ rdf:type bind:AssociationQualifier ;
    bind:onProperty liso:resultStatus ;
    bind:associationType bind:Aggregation
  ], 
  [ rdf:type bind:AssociationQualifier ;
    bind:onProperty liso:resultScoreConstraints ;
    bind:associationType bind:Aggregation
  ] .
liso:LineItem rdf:type bind:Addressable .
liso:LineItem rdfs:subClassOf
  [ rdf:type bind:AssociationQualifier ;
    bind:onProperty liso:reportingMethod ;
    bind:associationType bind:Aggregation
  ], 
  [ rdf:type bind:AssociationQualifier ;
    bind:onProperty liso:result ;
    bind:associationType bind:Composition
  ], 
  [ rdf:type bind:AssociationQualifier ;
    bind:onProperty liso:scoreConstraints ;
    bind:associationType bind:Aggregation
  ], 
  [ rdf:type bind:AssociationQualifier ;
    bind:onProperty liso:results ;
    bind:associationType bind:Composition
  ], 
  [ rdf:type bind:AssociationQualifier ;
    bind:onProperty liso:assignedActivity ;
    bind:associationType bind:Aggregation
  ], 
  [ rdf:type bind:AssociationQualifier ;
    bind:onProperty liso:dataSource
  ] .
liso:ScoreConstraints rdf:type bind:Addressable .
liso:ScoreConstraints rdf:type bind:AbstractClass .
liso:NumericLimits rdf:type bind:Addressable .
liso:ResultContainer rdf:type bind:Addressable .
liso:LineItemContainer rdf:type bind:Addressable .
liso:Result rdf:type bind:Addressable .
liso:ResultStatus rdf:type bind:Enum .
liso:AbstractResult rdf:type bind:Addressable .
liso:AbstractResult rdf:type bind:AbstractClass .
liso:AbstractResult rdfs:subClassOf
  [ rdf:type bind:AssociationQualifier ;
    bind:onProperty liso:resultAgent ;
    bind:associationType bind:Aggregation
  ], 
  [ rdf:type bind:AssociationQualifier ;
    bind:onProperty liso:gradedBy ;
    bind:associationType bind:Aggregation
  ] .
@prefix liss: <http://ld.kinexis.com/vocab/lis/v2/status#> .
@prefix owl: <http://www.w3.org/2002/07/owl#> .
@prefix rdf: <http://www.w3.org/1999/02/22-rdf-syntax-ns#> .
@prefix rdfs: <http://www.w3.org/2000/01/rdf-schema#> .
@prefix xsd: <http://www.w3.org/2001/XMLSchema#> .
@prefix bind: <http://purl.org/semantictools/v1/vocab/bind#> .

<http://ld.kinexis.com/vocab/lis/v2/status#> a owl:Ontology  ;
  rdfs:label "LIS Statuses" ;
  a bind:TargetNamespace ;
  bind:suggestedPrefix "liss" .

liss:LISStatus rdf:type owl:Class ; 
  rdfs:comment "Possible status values for LIS entities." .

liss:Active rdf:type liss:LISStatus .

liss:Inactive rdf:type liss:LISStatus .

liss:Deleted rdf:type liss:LISStatus .
@prefix rdf: <http://www.w3.org/1999/02/22-rdf-syntax-ns#> .
@prefix rdfs: <http://www.w3.org/2000/01/rdf-schema#> .
@prefix bind: <http://purl.org/semantictools/v1/vocab/bind#> .
@prefix liss: <http://ld.kinexis.com/vocab/lis/v2/status#> .

liss:LISStatus rdf:type bind:Enum .
@prefix schema: <http://schema.org/> .
@prefix org: <http://www.w3.org/ns/org#> .
@prefix xsd: <http://www.w3.org/2001/XMLSchema#> .
@prefix foaf: <http://xmlns.com/foaf/0.1#> .
@prefix owl: <http://www.w3.org/2002/07/owl#> .
@prefix rdf: <http://www.w3.org/1999/02/22-rdf-syntax-ns#> .
@prefix rdfs: <http://www.w3.org/2000/01/rdf-schema#> .
@prefix bind: <http://purl.org/semantictools/v1/vocab/bind#> .

<http://schema.org/> a owl:Ontology  ;
  rdfs:label "Schema.org Ontology" ;
  a bind:TargetNamespace ;
  bind:suggestedPrefix "schema" .

schema:Person rdf:type owl:Class ;
  rdfs:subClassOf foaf:Agent ,
  [ a owl:Restriction ;
    owl:onProperty      schema:name;
    owl:allValuesFrom  xsd:string;
    rdfs:comment "The person's assigned full name (typically their first name followed by their family name separated with a space)."
  ] ,
  [ a owl:Restriction ;
    owl:onProperty      schema:givenName;
    rdfs:comment "The person's assigned first name."
  ] ,
  [ a owl:Restriction ;
    owl:onProperty      schema:familyName;
    rdfs:comment "The person's assigned family name."
  ] ,
  [ a owl:Restriction ;
    owl:onProperty      schema:img;
    rdfs:comment "A URL to an image for the person."
  ] ; 
  rdfs:comment "A container for all the information about a single person." .

schema:name rdf:type owl:FunctionalProperty ;
  rdfs:domain  [
    rdf:type owl:Class ;
    owl:unionOf (
      schema:Person
      org:Organization
    )
  ] ;
  rdfs:range  [
    rdf:type owl:Class ;
    owl:unionOf (
      xsd:string
      xsd:string
    )
  ] ;
  rdfs:comment "The person's assigned full name (typically their first name followed by their family name separated with a space)." .

schema:givenName rdf:type owl:FunctionalProperty ;
  rdfs:domain schema:Person ;
  rdfs:range xsd:string ;
  rdfs:comment "The person's assigned first name." .

schema:familyName rdf:type owl:FunctionalProperty ;
  rdfs:domain schema:Person ;
  rdfs:range xsd:string ;
  rdfs:comment "The person's assigned family name." .

schema:img rdf:type owl:FunctionalProperty ;
  rdfs:domain schema:Person ;
  rdfs:range xsd:string ;
  rdfs:comment "A URL to an image for the person." .
@prefix rdf: <http://www.w3.org/1999/02/22-rdf-syntax-ns#> .
@prefix rdfs: <http://www.w3.org/2000/01/rdf-schema#> .
@prefix bind: <http://purl.org/semantictools/v1/vocab/bind#> .
@prefix schema: <http://schema.org/> .

schema:Person rdf:type bind:Addressable .
@prefix org: <http://www.w3.org/ns/org#> .
@prefix foaf: <http://xmlns.com/foaf/0.1#> .
@prefix lism: <http://ld.kinexis.com/vocab/lis/v2/mm#> .
@prefix liss: <http://ld.kinexis.com/vocab/lis/v2/status#> .
@prefix xsd: <http://www.w3.org/2001/XMLSchema#> .
@prefix schema: <http://schema.org/> .
@prefix owl: <http://www.w3.org/2002/07/owl#> .
@prefix rdf: <http://www.w3.org/1999/02/22-rdf-syntax-ns#> .
@prefix rdfs: <http://www.w3.org/2000/01/rdf-schema#> .
@prefix bind: <http://purl.org/semantictools/v1/vocab/bind#> .

<http://www.w3.org/ns/org#> a owl:Ontology  ;
  rdfs:label "W3C Organization" ;
  a bind:TargetNamespace ;
  bind:suggestedPrefix "org" .

org:Organization rdf:type owl:Class;
  rdfs:subClassOf 
  [ a owl:Restriction ;
    owl:onProperty      schema:name;
    owl:allValuesFrom  xsd:string;
    rdfs:comment "The organization's assigned name."
  ] ,
  [ a owl:Restriction ;
    owl:onProperty      org:membership;
    rdfs:comment "A membership entity that records the role of some Agent within this Organization."
  ] ,
  [ a owl:Restriction ;
    owl:onProperty      org:memberships;
    rdfs:comment "The container holding the LISMemberhips for this Organization."
  ] ; 
  rdfs:comment "A collection of people organized together into a community or other social, commercial or political structure.  The group has some common purpose or reason for existence which goes beyond the set of people belonging to it and can act as an Agent. Organizations are often decomposable into hierarchical structures." .

org:Membership rdf:type owl:Class;
  rdfs:subClassOf 
  [ a owl:Restriction ;
    owl:onProperty      org:status;
    rdfs:comment "The current status of a membership which applies to all roles."
  ] ,
  [ a owl:Restriction ;
    owl:onProperty      org:member;
    owl:minCardinality  1;
    rdfs:comment "Indicates the Person (or other Agent including Organization) involved in the Membership relationship."
  ] ,
  [ a owl:Restriction ;
    owl:onProperty      org:role;
    owl:minCardinality  1;
    rdfs:comment "Indicates the Role that the Agent plays in a Membership relationship with an Organization."
  ] ,
  [ a owl:Restriction ;
    owl:onProperty      org:organization;
    owl:minCardinality  1;
    rdfs:comment "Indicates the organization in which the Agent is a member."
  ] ; 
  rdfs:comment "Indicates the nature of an Agent's membership within an Organization." .

org:Role rdf:type owl:Class ; 
  rdfs:comment "Designates the role that a Person or other Agent can take in an organization." .

org:hasMembership rdf:type rdf:Property ;
  rdfs:domain foaf:Agent ;
  rdfs:range org:Membership ;
  owl:inverseOf org:member ;
  rdfs:comment "Indicates a membership relationship that the Agent plays." .

org:membership rdf:type rdf:Property ;
  rdfs:domain org:Organization ;
  rdfs:range org:Membership ;
  owl:inverseOf org:organization ;
  rdfs:comment "A membership entity that records the role of some Agent within this Organization." .

org:memberships rdf:type owl:FunctionalProperty ;
  rdfs:domain org:Organization ;
  rdfs:range lism:LISMembershipContainer ;
  rdfs:comment "The container holding the LISMemberhips for this Organization." .

org:status rdf:type owl:FunctionalProperty ;
  rdfs:domain org:Membership ;
  rdfs:range liss:LISStatus ;
  rdfs:comment "The current status of a membership which applies to all roles." .

org:member rdf:type owl:FunctionalProperty ;
  rdfs:domain org:Membership ;
  rdfs:range foaf:Agent ;
  owl:inverseOf org:hasMembership ;
  rdfs:comment "Indicates the Person (or other Agent including Organization) involved in the Membership relationship." .

org:role rdf:type rdf:Property ;
  rdfs:domain org:Membership ;
  rdfs:range org:Role ;
  rdfs:comment "Indicates the Role that the Agent plays in a Membership relationship with an Organization." .

org:organization rdf:type owl:FunctionalProperty ;
  rdfs:domain org:Membership ;
  rdfs:range org:Organization ;
  owl:inverseOf org:membership ;
  rdfs:comment "Indicates the organization in which the Agent is a member." .
@prefix rdf: <http://www.w3.org/1999/02/22-rdf-syntax-ns#> .
@prefix rdfs: <http://www.w3.org/2000/01/rdf-schema#> .
@prefix bind: <http://purl.org/semantictools/v1/vocab/bind#> .
@prefix org: <http://www.w3.org/ns/org#> .

org:Organization rdf:type bind:Addressable .
org:Organization rdf:type bind:AbstractClass .
org:Organization rdfs:subClassOf
  [ rdf:type bind:AssociationQualifier ;
    bind:onProperty org:memberships ;
    bind:associationType bind:Composition
  ] .
org:Membership rdf:type bind:Addressable .
org:Membership rdf:type bind:AbstractClass .
org:Membership rdfs:subClassOf
  [ rdf:type bind:AssociationQualifier ;
    bind:onProperty org:role
  ] .
org:Role rdf:type bind:Addressable .
org:Role rdf:type bind:AbstractClass .
@prefix lism: <http://ld.kinexis.com/vocab/lis/v2/mm#> .
@prefix org: <http://www.w3.org/ns/org#> .
@prefix ldp: <http://www.w3.org/ns/ldp#> .
@prefix owl: <http://www.w3.org/2002/07/owl#> .
@prefix rdf: <http://www.w3.org/1999/02/22-rdf-syntax-ns#> .
@prefix rdfs: <http://www.w3.org/2000/01/rdf-schema#> .
@prefix xsd: <http://www.w3.org/2001/XMLSchema#> .
@prefix bind: <http://purl.org/semantictools/v1/vocab/bind#> .

<http://ld.kinexis.com/vocab/lis/v2/mm#> a owl:Ontology  ;
  rdfs:label "LIS Membership Management" ;
  a bind:TargetNamespace ;
  bind:suggestedPrefix "lism" .

lism:LISMembershipContainer rdf:type owl:Class ;
  rdfs:subClassOf ldp:Container ,
  [ a owl:Restriction ;
    owl:onProperty      ldp:membershipPredicate;
    owl:hasValue org:membership
  ] ,
  [ a owl:Restriction ;
    owl:onProperty      ldp:membershipSubject;
    owl:allValuesFrom  org:Organization
  ] ; 
  rdfs:comment "A container that holds a collection of Membership resources." .

lism:LISRole rdf:type rdf:Property, org:Role ;
  rdfs:comment "A Role that is also a Property whose domain is restricted to the Organization class and whose range is restricted to the Person class." .

lism:Learner rdf:type rdf:Property ;
  rdfs:subPropertyOf lism:LISRole .

lism:Instructor rdf:type rdf:Property ;
  rdfs:subPropertyOf lism:LISRole .

lism:TeachingAssistant rdf:type rdf:Property ;
  rdfs:subPropertyOf lism:LISRole .

lism:NonCreditLearner rdf:type rdf:Property ;
  rdfs:subPropertyOf lism:Learner .

lism:GuestLearner rdf:type rdf:Property ;
  rdfs:subPropertyOf lism:Learner .

lism:ExternalLearner rdf:type rdf:Property ;
  rdfs:subPropertyOf lism:Learner .

lism:PrimaryInstructor rdf:type rdf:Property ;
  rdfs:subPropertyOf lism:Instructor .

lism:SecondaryInstructor rdf:type rdf:Property ;
  rdfs:subPropertyOf lism:Instructor .

lism:Lecturer rdf:type rdf:Property ;
  rdfs:subPropertyOf lism:Instructor .

lism:GuestInstructor rdf:type rdf:Property ;
  rdfs:subPropertyOf lism:Instructor .

lism:ExternalInstructor rdf:type rdf:Property ;
  rdfs:subPropertyOf lism:Instructor .
@prefix rdf: <http://www.w3.org/1999/02/22-rdf-syntax-ns#> .
@prefix rdfs: <http://www.w3.org/2000/01/rdf-schema#> .
@prefix bind: <http://purl.org/semantictools/v1/vocab/bind#> .
@prefix lism: <http://ld.kinexis.com/vocab/lis/v2/mm#> .

lism:LISMembershipContainer rdf:type bind:Addressable .
@prefix owl: <http://www.w3.org/2002/07/owl#> .
@prefix bind: <http://purl.org/semantictools/v1/vocab/bind#> .

<http://ld.kinexis.com/xsd/lti/v2/ltid#> a owl:Ontology ;
  bind:suggestedPrefix "lti-type" .


